partial locale refactor

Abstract_Value_Flow_Analysis.thy
@@ -15,6 +15,1270 @@ fun site_set :: "exp \<Rightarrow> (var + var) set" where
   "site_set (LET x = SPAWN _ in _) = {Inl x, Inr x}" |
   "site_set (LET x = _ in e) = {Inl x}"
 
+locale flow_analysis = 
+  fixes 
+    let_unit :: "'a \<Rightarrow> abstract_value_env \<Rightarrow> var \<Rightarrow> exp \<Rightarrow> bool" and 
+    let_abs :: "'a \<Rightarrow> abstract_value_env \<Rightarrow> var \<Rightarrow> (var \<times> var \<times> exp) \<Rightarrow> exp \<Rightarrow> bool" and 
+    let_pair :: "'a \<Rightarrow> abstract_value_env \<Rightarrow> var \<Rightarrow> (var \<times> var) \<Rightarrow> exp \<Rightarrow> bool" and 
+    let_left :: "'a \<Rightarrow> abstract_value_env \<Rightarrow> var \<Rightarrow> var \<Rightarrow> exp \<Rightarrow> bool" and 
+    let_right :: "'a \<Rightarrow> abstract_value_env \<Rightarrow> var \<Rightarrow> var \<Rightarrow> exp \<Rightarrow> bool" and 
+    let_send_evt :: "'a \<Rightarrow> abstract_value_env \<Rightarrow> var \<Rightarrow> (var \<times> var) \<Rightarrow> exp \<Rightarrow> bool" and 
+    let_recv_evt :: "'a \<Rightarrow> abstract_value_env \<Rightarrow> var \<Rightarrow> var \<Rightarrow> exp \<Rightarrow> bool" and 
+    let_case :: "'a \<Rightarrow> abstract_value_env \<Rightarrow> var \<Rightarrow> (var \<times> var \<times> exp \<times> var \<times> exp) \<Rightarrow> exp \<Rightarrow> bool" and 
+    let_fst :: "'a \<Rightarrow> abstract_value_env \<Rightarrow> var \<Rightarrow> var \<Rightarrow> exp \<Rightarrow> bool" and 
+    let_snd :: "'a \<Rightarrow> abstract_value_env \<Rightarrow> var \<Rightarrow> var \<Rightarrow> exp \<Rightarrow> bool" and 
+    let_app :: "'a \<Rightarrow> abstract_value_env \<Rightarrow> var \<Rightarrow> (var \<times> var) \<Rightarrow> exp \<Rightarrow> bool" and 
+    let_sync :: "'a \<Rightarrow> abstract_value_env \<Rightarrow> var \<Rightarrow> var \<Rightarrow> exp \<Rightarrow> bool" and 
+    let_chan :: "'a \<Rightarrow> abstract_value_env \<Rightarrow> var \<Rightarrow> exp \<Rightarrow> bool" and 
+    let_spawn :: "'a \<Rightarrow> abstract_value_env \<Rightarrow> var \<Rightarrow> exp \<Rightarrow> exp \<Rightarrow> bool"
+
+context flow_analysis
+begin
+
+inductive accept_exp :: "'a \<times> abstract_value_env \<Rightarrow> exp \<Rightarrow> bool" (infix "\<Turnstile>\<^sub>e" 55) where
+  Result: "
+    (\<G>, \<V>) \<Turnstile>\<^sub>e (RESULT x)
+  " |
+  Let_Unit: "
+    \<lbrakk> 
+      let_unit \<G> \<V> x e;
+      (\<G>, \<V>) \<Turnstile>\<^sub>e e
+    \<rbrakk> \<Longrightarrow> 
+    (\<G>, \<V>) \<Turnstile>\<^sub>e LET x = \<lparr>\<rparr> in e
+  " |
+  Let_Abs : "
+    \<lbrakk>
+      let_abs \<G> \<V> x (f', x', e') e;
+      (\<G>, \<V>) \<Turnstile>\<^sub>e e';
+      (\<G>, \<V>) \<Turnstile>\<^sub>e e 
+    \<rbrakk> \<Longrightarrow> 
+    (\<G>, \<V>) \<Turnstile>\<^sub>e LET x = FN f' x' . e' in e
+  " |
+  Let_Pair : "
+    \<lbrakk> 
+      let_pair \<G> \<V> x (x\<^sub>1, x\<^sub>2) e;
+      (\<G>, \<V>) \<Turnstile>\<^sub>e e 
+    \<rbrakk> \<Longrightarrow> 
+    (\<G>, \<V>) \<Turnstile>\<^sub>e LET x = \<lparr>x\<^sub>1, x\<^sub>2\<rparr> in e
+  " |
+  Let_Left : "
+    \<lbrakk>
+      let_left \<G> \<V> x x\<^sub>l e;
+      (\<G>, \<V>) \<Turnstile>\<^sub>e e 
+    \<rbrakk> \<Longrightarrow> 
+    (\<G>, \<V>) \<Turnstile>\<^sub>e LET x = LEFT x\<^sub>l in e
+  " |
+  Let_Right : "
+    \<lbrakk>
+      let_right \<G> \<V> x x\<^sub>r e;
+      (\<G>, \<V>) \<Turnstile>\<^sub>e e
+    \<rbrakk> \<Longrightarrow> 
+    (\<G>, \<V>) \<Turnstile>\<^sub>e LET x = RIGHT x\<^sub>r in e
+  " |
+  Let_Send_Evt : "
+    \<lbrakk> 
+      let_send_evt \<G> \<V> x (x\<^sub>c, x\<^sub>m) e;
+      (\<G>, \<V>) \<Turnstile>\<^sub>e e 
+    \<rbrakk> \<Longrightarrow> 
+    (\<G>, \<V>) \<Turnstile>\<^sub>e LET x = SEND EVT x\<^sub>c x\<^sub>m in e
+  " |
+  Let_Recv_Evt : "
+    \<lbrakk> 
+      let_recv_evt \<G> \<V> x x\<^sub>c e;
+      (\<G>, \<V>) \<Turnstile>\<^sub>e e 
+    \<rbrakk> \<Longrightarrow> 
+    (\<G>, \<V>) \<Turnstile>\<^sub>e LET x = RECV EVT x\<^sub>c in e
+  " |
+  Let_Case: "
+    \<lbrakk>
+      let_case \<G> \<V> x (x\<^sub>s, x\<^sub>l, e\<^sub>l, x\<^sub>r, e\<^sub>r) e;
+      (\<G>, \<V>) \<Turnstile>\<^sub>e e
+    \<rbrakk> \<Longrightarrow> 
+    (\<G>, \<V>) \<Turnstile>\<^sub>e LET x = CASE x\<^sub>s LEFT x\<^sub>l |> e\<^sub>l RIGHT x\<^sub>r |> e\<^sub>r in e
+  "|
+  Let_Fst: "
+    \<lbrakk> 
+      let_fst \<G> \<V> x x\<^sub>p e;
+      (\<G>, \<V>) \<Turnstile>\<^sub>e e 
+    \<rbrakk> \<Longrightarrow> 
+    (\<G>, \<V>) \<Turnstile>\<^sub>e LET x = FST x\<^sub>p in e
+  " |
+  Let_Snd: "
+    \<lbrakk> 
+      let_snd \<G> \<V> x x\<^sub>p e;
+      (\<G>, \<V>) \<Turnstile>\<^sub>e e
+    \<rbrakk> \<Longrightarrow> 
+    (\<G>, \<V>) \<Turnstile>\<^sub>e LET x = SND x\<^sub>p in e
+  " |
+  Let_App: "
+    \<lbrakk>
+      let_app \<G> \<V> x (f, x\<^sub>a) e;
+      (\<G>, \<V>) \<Turnstile>\<^sub>e e
+    \<rbrakk> \<Longrightarrow> 
+    (\<G>, \<V>) \<Turnstile>\<^sub>e LET x = APP f x\<^sub>a in e
+  " |
+  Let_Sync  : "
+    \<lbrakk> 
+      let_sync \<G> \<V> x x\<^sub>e e;
+      (\<G>, \<V>) \<Turnstile>\<^sub>e e
+    \<rbrakk> \<Longrightarrow>  
+    (\<G>, \<V>) \<Turnstile>\<^sub>e LET x = SYNC x\<^sub>e in e
+  " |
+  Let_Chan: "
+    \<lbrakk>
+      let_chan \<G> \<V> x e;
+      (\<G>, \<V>) \<Turnstile>\<^sub>e e
+    \<rbrakk> \<Longrightarrow>  
+    (\<G>, \<V>) \<Turnstile>\<^sub>e LET x = CHAN \<lparr>\<rparr> in e
+  " |
+  Let_Spawn: "
+    \<lbrakk>
+      let_spawn \<G> \<V> x e\<^sub>c e;
+      (\<G>, \<V>) \<Turnstile>\<^sub>e e\<^sub>c;
+      (\<G>, \<V>) \<Turnstile>\<^sub>e e
+    \<rbrakk> \<Longrightarrow>  
+    (\<G>, \<V>) \<Turnstile>\<^sub>e LET x = SPAWN e\<^sub>c in e
+  "
+
+
+fun value_to_abstract_value :: "val \<Rightarrow> abstract_value" ("|_|" [0]61) where
+  "|\<lbrace>Ch \<pi> x\<rbrace>| = ^Chan x" |
+  "|\<lbrace>p, \<rho>\<rbrace>| = ^p" |
+  "|\<lbrace>\<rbrace>| = ^\<lparr>\<rparr>"
+
+definition env_to_abstract_value_env :: "(var \<rightharpoonup> val) \<Rightarrow> abstract_value_env" ("\<parallel>_\<parallel>" [0]61) where
+  "\<parallel>\<rho>\<parallel> = (\<lambda> x . (case (\<rho> x) of 
+    Some \<omega> \<Rightarrow> {|\<omega>|} |
+    None \<Rightarrow> {}
+  ))"
+
+definition abstract_value_env_precision :: "abstract_value_env \<Rightarrow> abstract_value_env \<Rightarrow> bool" (infix "\<sqsubseteq>" 55) where
+  "\<V> \<sqsubseteq> \<V>' \<equiv> (\<forall> x . \<V> x \<subseteq> \<V>' x)"
+
+
+inductive accept_value :: "'a \<times> abstract_value_env \<Rightarrow> val \<Rightarrow> bool" (infix "\<Turnstile>\<^sub>\<omega>" 55)
+and  accept_val_env :: "'a \<times> abstract_value_env \<Rightarrow> val_env \<Rightarrow> bool" (infix "\<Turnstile>\<^sub>\<rho>" 55) 
+where
+  Unit: "(\<G>, \<V>) \<Turnstile>\<^sub>\<omega> \<lbrace>\<rbrace>" |
+  Chan: "(\<G>, \<V>) \<Turnstile>\<^sub>\<omega> \<lbrace>c\<rbrace>" |
+  Abs: "
+    \<lbrakk>
+      {^Abs f x e} \<subseteq> \<V> f;
+      (\<G>, \<V>) \<Turnstile>\<^sub>e e;
+      (\<G>, \<V>) \<Turnstile>\<^sub>\<rho> \<rho>
+    \<rbrakk> \<Longrightarrow> 
+    (\<G>, \<V>) \<Turnstile>\<^sub>\<omega> \<lbrace>Abs f x e, \<rho>\<rbrace>
+  " |
+  Pair: "
+    (\<G>, \<V>) \<Turnstile>\<^sub>\<rho> \<rho>
+    \<Longrightarrow>
+    (\<G>, \<V>) \<Turnstile>\<^sub>\<omega> \<lbrace>Pair _ _, \<rho>\<rbrace>
+  " |
+  Left: "
+    (\<G>, \<V>) \<Turnstile>\<^sub>\<rho> \<rho>
+    \<Longrightarrow>
+    (\<G>, \<V>) \<Turnstile>\<^sub>\<omega> \<lbrace>Left _, \<rho>\<rbrace>
+  " |
+  Right: "
+    (\<G>, \<V>) \<Turnstile>\<^sub>\<rho> \<rho>
+    \<Longrightarrow>
+    (\<G>, \<V>) \<Turnstile>\<^sub>\<omega> \<lbrace>Right _, \<rho>\<rbrace>
+  " |
+  Send_Evt: "
+    (\<G>, \<V>) \<Turnstile>\<^sub>\<rho> \<rho>
+    \<Longrightarrow>
+    (\<G>, \<V>) \<Turnstile>\<^sub>\<omega> \<lbrace>Send_Evt _ _, \<rho>\<rbrace>
+  " |
+  Recv_Evt: "
+    (\<G>, \<V>) \<Turnstile>\<^sub>\<rho> \<rho>
+    \<Longrightarrow>
+    (\<G>, \<V>) \<Turnstile>\<^sub>\<omega> \<lbrace>Recv_Evt _, \<rho>\<rbrace>
+  " |
+  Always_Evt: "
+    (\<G>, \<V>) \<Turnstile>\<^sub>\<rho> \<rho>
+    \<Longrightarrow>
+    (\<G>, \<V>) \<Turnstile>\<^sub>\<omega> \<lbrace>Always_Evt _, \<rho>\<rbrace>
+  " |
+
+  Any : "
+    \<lbrakk>
+      (\<forall> x \<omega> . \<rho> x = Some \<omega> \<longrightarrow>
+        {|\<omega>|} \<subseteq> \<V> x \<and> (\<G>, \<V>) \<Turnstile>\<^sub>\<omega> \<omega>
+      )
+    \<rbrakk> \<Longrightarrow>
+    (\<G>, \<V>) \<Turnstile>\<^sub>\<rho> \<rho>
+  "
+
+
+inductive accept_stack :: "'a \<times> abstract_value_env \<Rightarrow> abstract_value set \<Rightarrow> cont list \<Rightarrow> bool" ("_ \<Turnstile>\<^sub>\<kappa> _ \<Rrightarrow> _" [56,0,56]55) where
+  Empty: "(\<G>, \<V>) \<Turnstile>\<^sub>\<kappa> \<W> \<Rrightarrow> []" |
+  Nonempty: "
+    \<lbrakk> 
+      \<W> \<subseteq> \<V> x;
+      (\<G>, \<V>) \<Turnstile>\<^sub>e e;
+      (\<G>, \<V>) \<Turnstile>\<^sub>\<rho> \<rho>;
+      (\<G>, \<V>) \<Turnstile>\<^sub>\<kappa> \<V> (\<lfloor>e\<rfloor>) \<Rrightarrow> \<kappa>
+    \<rbrakk> \<Longrightarrow> 
+    (\<G>, \<V>) \<Turnstile>\<^sub>\<kappa> \<W> \<Rrightarrow> (\<langle>x, e, \<rho>\<rangle> # \<kappa>)
+  "
+
+
+inductive accept_state :: "'a \<times> abstract_value_env \<Rightarrow> state \<Rightarrow> bool" (infix "\<Turnstile>\<^sub>\<sigma>" 55)  where
+  Any: "
+    \<lbrakk>
+      (\<G>, \<V>) \<Turnstile>\<^sub>e e;
+      (\<G>, \<V>) \<Turnstile>\<^sub>\<rho> \<rho>;
+      (\<G>, \<V>) \<Turnstile>\<^sub>\<kappa> \<V> (\<lfloor>e\<rfloor>) \<Rrightarrow> \<kappa>
+    \<rbrakk> \<Longrightarrow>
+    (\<G>, \<V>) \<Turnstile>\<^sub>\<sigma> \<langle>e; \<rho>; \<kappa>\<rangle>
+  "
+
+inductive accept_state_pool :: "'a \<times> abstract_value_env \<Rightarrow> state_pool \<Rightarrow> bool" (infix "\<Turnstile>\<^sub>\<E>" 55) where
+  Any: "
+    (\<forall> \<pi> \<sigma> . \<E> \<pi> = Some \<sigma> \<longrightarrow> (\<G>, \<V>) \<Turnstile>\<^sub>\<sigma> \<sigma>)
+    \<Longrightarrow> 
+    (\<G>, \<V>) \<Turnstile>\<^sub>\<E> \<E>
+  "
+
+
+(*******Soundness*****)
+
+(*
+*)
+lemma flow_state_to_flow_exp: "
+  (\<G>, \<V>) \<Turnstile>\<^sub>\<sigma> \<langle>RESULT x;\<rho>;\<langle>x\<^sub>\<kappa>,e\<^sub>\<kappa>,\<rho>\<^sub>\<kappa>\<rangle> # \<kappa>\<rangle> \<Longrightarrow> \<rho> x = Some \<omega> \<Longrightarrow> (\<G>, \<V>) \<Turnstile>\<^sub>e  e\<^sub>\<kappa>
+"
+ apply (erule accept_state.cases, auto)
+ apply (erule accept_stack.cases, auto)
+done
+
+lemma flow_over_state_to_env: "
+  (\<G>, \<V>) \<Turnstile>\<^sub>\<sigma>  \<langle>RESULT x; \<rho>; \<langle>x\<^sub>\<kappa>,e\<^sub>\<kappa>,\<rho>\<^sub>\<kappa>\<rangle> # \<kappa>\<rangle> \<Longrightarrow> \<rho> x = Some \<omega> \<Longrightarrow> 
+  (\<G>, \<V>) \<Turnstile>\<^sub>\<rho> \<rho>\<^sub>\<kappa>(x\<^sub>\<kappa> \<mapsto> \<omega>)
+"
+ apply (rule accept_value_accept_val_env.Any, auto)
+      apply (erule accept_state.cases, auto)
+      apply (erule accept_val_env.cases, auto)
+      apply (erule accept_stack.cases, auto)
+     apply (erule accept_state.cases, auto)
+     apply (erule accept_val_env.cases, auto)
+    apply (rename_tac x' \<omega>')
+    apply (erule accept_state.cases, auto)
+    apply (erule accept_val_env.cases, auto)
+    apply (drule spec[of _ x]; auto)
+     apply (erule accept_stack.cases; auto)+
+    apply (erule accept_val_env.cases; auto)+
+   apply (rename_tac x' \<omega>')
+   apply (erule accept_state.cases, auto)
+   apply (erule accept_val_env.cases, auto)
+   apply (drule spec[of _ x]; auto)
+    apply (erule accept_stack.cases; auto)+
+   apply (erule accept_val_env.cases; auto)+
+done
+
+lemma flow_over_state_to_stack: "
+  (\<G>, \<V>) \<Turnstile>\<^sub>\<sigma>  \<langle>RESULT x; \<rho>; \<langle>x\<^sub>\<kappa>,e\<^sub>\<kappa>,\<rho>\<^sub>\<kappa>\<rangle> # \<kappa>\<rangle> \<Longrightarrow> \<rho> x = Some \<omega> \<Longrightarrow> (\<G>, \<V>) \<Turnstile>\<^sub>\<kappa>  \<V> (\<lfloor>e\<^sub>\<kappa>\<rfloor>) \<Rrightarrow> \<kappa>
+"
+ apply (erule accept_state.cases, auto)
+ apply (erule accept_val_env.cases, auto)
+ apply (drule spec)+
+ apply (erule impE, auto)
+ apply (erule accept_stack.cases, auto)+
+done
+
+lemma flow_over_state_1: "
+  (\<G>, \<V>) \<Turnstile>\<^sub>\<sigma>  \<langle>RESULT x; \<rho>; \<langle>x\<^sub>\<kappa>,e\<^sub>\<kappa>,\<rho>\<^sub>\<kappa>\<rangle> # \<kappa>\<rangle> \<Longrightarrow> \<rho> x = Some \<omega> \<Longrightarrow> (\<G>, \<V>) \<Turnstile>\<^sub>\<sigma>  \<langle>e\<^sub>\<kappa>; \<rho>\<^sub>\<kappa>(x\<^sub>\<kappa> \<mapsto> \<omega>); \<kappa>\<rangle>
+"
+ apply (rule accept_state.Any)
+    apply (erule flow_state_to_flow_exp, auto)
+   apply (erule flow_over_state_to_env, auto)
+  apply (erule flow_over_state_to_stack, auto)
+done
+
+lemma flow_state_to_flow_exp_2: "
+  (\<G>, \<V>) \<Turnstile>\<^sub>\<sigma>  \<langle>LET x = \<lparr>\<rparr> in e; \<rho>; \<kappa>\<rangle> \<Longrightarrow> (\<G>, \<V>) \<Turnstile>\<^sub>e  e
+"
+ apply (erule accept_state.cases, auto)
+ apply (erule accept_exp.cases, auto)
+done
+
+
+lemma flow_over_state_to_env_2: "
+  (\<G>, \<V>) \<Turnstile>\<^sub>\<sigma>  \<langle>LET x = \<lparr>\<rparr> in e; \<rho>; \<kappa>\<rangle> \<Longrightarrow> (\<G>, \<V>) \<Turnstile>\<^sub>\<rho> \<rho>(x \<mapsto> \<lbrace>\<rbrace>)
+"
+ apply (rule accept_value_accept_val_env.Any, auto)
+     apply (erule accept_state.cases, auto)
+     apply (erule accept_exp.cases, auto)
+    apply (rule accept_value_accept_val_env.Unit)
+   apply (rename_tac x' \<omega>')
+   apply (erule accept_state.cases, auto)
+   apply (erule accept_val_env.cases, auto)
+  apply (erule accept_state.cases, auto)
+ apply (erule accept_val_env.cases, auto)
+sorry
+
+lemma flow_over_state_to_stack_2: "
+  (\<G>, \<V>) \<Turnstile>\<^sub>\<sigma>  \<langle>LET x = \<lparr>\<rparr> in e; \<rho>; \<kappa>\<rangle> \<Longrightarrow> (\<G>, \<V>) \<Turnstile>\<^sub>\<kappa>  \<V> (\<lfloor>e\<rfloor>) \<Rrightarrow> \<kappa>
+"
+ apply (erule accept_state.cases, auto)
+done
+
+lemma flow_over_state_2: "
+  (\<G>, \<V>) \<Turnstile>\<^sub>\<sigma>  \<langle>LET x = \<lparr>\<rparr> in e; \<rho>; \<kappa>\<rangle> \<Longrightarrow> (\<G>, \<V>) \<Turnstile>\<^sub>\<sigma>  \<langle>e; \<rho>(x \<mapsto> \<lbrace>\<rbrace>); \<kappa>\<rangle>
+"
+ apply (rule accept_state.Any)
+    apply (erule flow_state_to_flow_exp_2)
+   apply (erule flow_over_state_to_env_2)
+  apply (erule flow_over_state_to_stack_2)
+done
+
+(*
+lemma flow_over_state_to_exp_3: "
+  (\<G>, \<V>) \<Turnstile>\<^sub>\<sigma>  \<langle>LET x = Prim p in e; \<rho>; \<kappa>\<rangle> \<Longrightarrow> (\<G>, \<V>) \<Turnstile>\<^sub>e  e
+"
+ apply (erule accept_state.cases, auto)  
+ apply (erule accept_exp.cases, auto)
+done
+
+lemma flow_over_state_to_env_3: "
+  (\<G>, \<V>) \<Turnstile>\<^sub>\<sigma>  \<langle>LET x = Prim p in e; \<rho>; \<kappa>\<rangle> \<Longrightarrow> (\<G>, \<V>) \<Turnstile>\<^sub>\<rho> \<rho>(x \<mapsto> \<lbrace>p, \<rho>\<rbrace>)
+"
+ apply (rule accept_value_accept_val_env.Any, auto)
+     apply (erule accept_state.cases, auto)
+     apply (erule accept_exp.cases, auto)
+    apply (erule accept_state.cases, auto)
+    apply ((erule accept_exp.cases, auto); rule, auto)
+   apply (rename_tac x' \<omega>')
+   apply (erule accept_state.cases, auto)
+   apply (erule accept_val_env.cases, auto)
+   apply (erule accept_state.cases, auto)
+  apply (erule accept_val_env.cases, auto)
+done
+
+lemma flow_over_state_to_stack_3: "
+  (\<G>, \<V>) \<Turnstile>\<^sub>\<sigma>  \<langle>LET x = Prim p in e; \<rho>; \<kappa>\<rangle> \<Longrightarrow> (\<G>, \<V>) \<Turnstile>\<^sub>\<kappa>  \<V> (\<lfloor>e\<rfloor>) \<Rrightarrow> \<kappa>
+"
+ apply (erule accept_state.cases, auto)
+done
+
+lemma flow_over_state_3: "
+  (\<G>, \<V>) \<Turnstile>\<^sub>\<sigma>  \<langle>LET x = Prim p in e; \<rho>; \<kappa>\<rangle> \<Longrightarrow>  (\<G>, \<V>) \<Turnstile>\<^sub>\<sigma>  \<langle>e; \<rho>(x \<mapsto> \<lbrace>p, \<rho>\<rbrace>); \<kappa>\<rangle>
+"
+ apply (rule accept_state.Any)
+    apply (erule flow_over_state_to_exp_3)
+   apply (erule flow_over_state_to_env_3)
+  apply (erule flow_over_state_to_stack_3)
+done
+
+lemma flow_state_to_flow_exp_4: "
+  (\<G>, \<V>) \<Turnstile>\<^sub>\<sigma>  \<langle>LET x = CASE x\<^sub>s LEFT x\<^sub>l |> e\<^sub>l RIGHT x\<^sub>r |> e\<^sub>r in e; \<rho>; \<kappa>\<rangle> \<Longrightarrow> 
+  \<rho> x\<^sub>s = Some \<lbrace>prim.Left x\<^sub>l', \<rho>\<^sub>l\<rbrace> \<Longrightarrow> 
+  \<rho>\<^sub>l x\<^sub>l' = Some \<omega>\<^sub>l \<Longrightarrow> (\<G>, \<V>) \<Turnstile>\<^sub>e  e\<^sub>l
+"
+ apply (erule accept_state.cases, auto)
+ apply (erule accept_exp.cases, auto)
+ apply (erule accept_val_env.cases, auto)
+ apply ((drule spec)+, auto)
+done
+
+lemma flow_state_to_flow_env_4: "
+  (\<G>, \<V>) \<Turnstile>\<^sub>\<sigma>  \<langle>LET x = CASE x\<^sub>s LEFT x\<^sub>l |> e\<^sub>l RIGHT x\<^sub>r |> e\<^sub>r in e; \<rho>; \<kappa>\<rangle> \<Longrightarrow> 
+  \<rho> x\<^sub>s = Some \<lbrace>prim.Left x\<^sub>l', \<rho>\<^sub>l\<rbrace> \<Longrightarrow> \<rho>\<^sub>l x\<^sub>l' = Some \<omega>\<^sub>l \<Longrightarrow> 
+  (\<G>, \<V>) \<Turnstile>\<^sub>\<rho> \<rho>(x\<^sub>l \<mapsto> \<omega>\<^sub>l)
+"
+ apply (rule accept_value_accept_val_env.Any, auto)
+      apply (erule accept_state.cases, auto)
+      apply (erule accept_val_env.cases, auto)
+      apply (drule spec[of _ x\<^sub>s]; auto)
+      apply (erule accept_value.cases, auto)
+      apply (erule accept_val_env.cases, auto)
+      apply (drule spec[of _ x\<^sub>l']; auto)
+      apply (erule accept_exp.cases, auto)
+     apply (erule accept_state.cases, auto)
+     apply (erule accept_val_env.cases, auto)
+     apply (drule spec[of _ x\<^sub>s]; auto)
+     apply (erule accept_value.cases, auto)
+     apply (erule accept_val_env.cases, auto)
+    apply (rename_tac x' \<omega>')
+    apply (erule accept_state.cases, auto)
+    apply (erule accept_val_env.cases, auto)
+   apply (rename_tac x' \<omega>')
+   apply (erule accept_state.cases, auto)
+   apply (erule accept_val_env.cases, auto)
+done
+
+lemma flow_state_to_flow_stack_4: "
+  (\<G>, \<V>) \<Turnstile>\<^sub>\<sigma>  \<langle>LET x = CASE x\<^sub>s LEFT x\<^sub>l |> e\<^sub>l RIGHT x\<^sub>r |> e\<^sub>r in e; \<rho>; \<kappa>\<rangle> \<Longrightarrow>
+  \<rho> x\<^sub>s = Some \<lbrace>prim.Left x\<^sub>l', \<rho>\<^sub>l\<rbrace> \<Longrightarrow> \<rho>\<^sub>l x\<^sub>l' = Some \<omega>\<^sub>l \<Longrightarrow> 
+  (\<G>, \<V>) \<Turnstile>\<^sub>\<kappa> \<V> (\<lfloor>e\<^sub>l\<rfloor>) \<Rrightarrow> \<langle>x,e,\<rho>\<rangle> # \<kappa>
+"
+ apply (rule accept_stack.Nonempty)
+    apply (erule accept_state.cases, auto, rename_tac \<omega>)
+    apply (erule accept_val_env.cases, auto)
+    apply (drule spec[of _ x\<^sub>s]; auto)
+    apply (erule accept_exp.cases, auto)
+   apply (erule accept_state.cases, auto)
+   apply (erule accept_exp.cases, auto)
+  apply (erule accept_state.cases, auto)
+ apply (erule accept_state.cases, auto)
+done
+
+lemma flow_over_state_4: "
+  (\<G>, \<V>) \<Turnstile>\<^sub>\<sigma>  \<langle>LET x = CASE x\<^sub>s LEFT x\<^sub>l |> e\<^sub>l RIGHT x\<^sub>r |> e\<^sub>r in e; \<rho>; \<kappa>\<rangle> \<Longrightarrow> 
+  \<rho> x\<^sub>s = Some \<lbrace>prim.Left x\<^sub>l', \<rho>\<^sub>l\<rbrace> \<Longrightarrow> 
+  \<rho>\<^sub>l x\<^sub>l' = Some \<omega>\<^sub>l \<Longrightarrow> (\<G>, \<V>) \<Turnstile>\<^sub>\<sigma>  \<langle>e\<^sub>l; \<rho>(x\<^sub>l \<mapsto> \<omega>\<^sub>l); \<langle>x,e,\<rho>\<rangle> # \<kappa>\<rangle>
+"
+ apply (rule accept_state.Any)
+    apply (erule flow_state_to_flow_exp_4, simp, auto)
+   apply (erule flow_state_to_flow_env_4, simp, auto)
+  apply (erule flow_state_to_flow_stack_4, simp, auto)
+done
+
+lemma flow_state_to_flow_exp_5: "
+  (\<G>, \<V>) \<Turnstile>\<^sub>\<sigma>  \<langle>LET x = CASE x\<^sub>s LEFT x\<^sub>l |> e\<^sub>l RIGHT x\<^sub>r |> e\<^sub>r in e; \<rho>; \<kappa>\<rangle> \<Longrightarrow> 
+  \<rho> x\<^sub>s = Some \<lbrace>prim.Right x\<^sub>r', \<rho>\<^sub>r\<rbrace> \<Longrightarrow> 
+  \<rho>\<^sub>r x\<^sub>r' = Some \<omega>\<^sub>r \<Longrightarrow> (\<G>, \<V>) \<Turnstile>\<^sub>e  e\<^sub>r
+"
+ apply (erule accept_state.cases, auto)
+ apply (erule accept_exp.cases, auto)
+ apply (erule accept_val_env.cases, auto)
+ apply ((drule spec)+, auto)
+done
+
+lemma flow_state_to_flow_env_5: "
+  (\<G>, \<V>) \<Turnstile>\<^sub>\<sigma>  \<langle>LET x = CASE x\<^sub>s LEFT x\<^sub>l |> e\<^sub>l RIGHT x\<^sub>r |> e\<^sub>r in e; \<rho>; \<kappa>\<rangle> \<Longrightarrow> 
+  \<rho> x\<^sub>s = Some \<lbrace>prim.Right x\<^sub>r', \<rho>\<^sub>r\<rbrace> \<Longrightarrow> \<rho>\<^sub>r x\<^sub>r' = Some \<omega>\<^sub>r \<Longrightarrow> 
+  (\<G>, \<V>) \<Turnstile>\<^sub>\<rho> \<rho>(x\<^sub>r \<mapsto> \<omega>\<^sub>r)
+"
+ apply (rule accept_value_accept_val_env.Any, auto)
+      apply (erule accept_state.cases, auto)
+      apply (erule accept_val_env.cases, auto)
+      apply (drule spec[of _ x\<^sub>s]; auto)
+      apply (erule accept_value.cases, auto)
+      apply (erule accept_val_env.cases, auto)
+      apply (drule spec[of _ x\<^sub>r']; auto)
+      apply (erule accept_exp.cases, auto)
+     apply (erule accept_state.cases, auto)
+     apply (erule accept_val_env.cases, auto)
+     apply (drule spec[of _ x\<^sub>s]; auto)
+     apply (erule accept_value.cases, auto)
+     apply (erule accept_val_env.cases, auto)
+    apply (rename_tac x' \<omega>')
+    apply (erule accept_state.cases, auto)
+    apply (erule accept_val_env.cases, auto)
+   apply (rename_tac x' \<omega>')
+   apply (erule accept_state.cases, auto)
+   apply (erule accept_val_env.cases, auto)
+done
+
+lemma flow_state_to_flow_stack_5: "
+  (\<G>, \<V>) \<Turnstile>\<^sub>\<sigma>  \<langle>LET x = CASE x\<^sub>s LEFT x\<^sub>l |> e\<^sub>l RIGHT x\<^sub>r |> e\<^sub>r in e; \<rho>; \<kappa>\<rangle> \<Longrightarrow>
+  \<rho> x\<^sub>s = Some \<lbrace>prim.Right x\<^sub>r', \<rho>\<^sub>r\<rbrace> \<Longrightarrow> \<rho>\<^sub>r x\<^sub>r' = Some \<omega>\<^sub>r \<Longrightarrow> 
+  (\<G>, \<V>) \<Turnstile>\<^sub>\<kappa>  \<V> (\<lfloor>e\<^sub>r\<rfloor>) \<Rrightarrow> \<langle>x,e,\<rho>\<rangle> # \<kappa>
+"
+ apply (rule accept_stack.Nonempty)
+    apply (erule accept_state.cases, auto, rename_tac \<omega>)
+    apply (erule accept_val_env.cases, auto)
+    apply (drule spec[of _ x\<^sub>s]; auto)
+    apply (erule accept_exp.cases, auto)
+   apply (erule accept_state.cases, auto)
+   apply (erule accept_exp.cases, auto)
+  apply (erule accept_state.cases, auto)
+ apply (erule accept_state.cases, auto)
+done
+
+lemma flow_over_state_5: "
+  (\<G>, \<V>) \<Turnstile>\<^sub>\<sigma>  \<langle>LET x = CASE x\<^sub>s LEFT x\<^sub>l |> e\<^sub>l RIGHT x\<^sub>r |> e\<^sub>r in e; \<rho>; \<kappa>\<rangle> \<Longrightarrow> 
+  \<rho> x\<^sub>s = Some \<lbrace>prim.Right x\<^sub>r', \<rho>\<^sub>r\<rbrace> \<Longrightarrow> 
+  \<rho>\<^sub>r x\<^sub>r' = Some \<omega>\<^sub>r \<Longrightarrow> (\<G>, \<V>) \<Turnstile>\<^sub>\<sigma>  \<langle>e\<^sub>r; \<rho>(x\<^sub>r \<mapsto> \<omega>\<^sub>r); \<langle>x,e,\<rho>\<rangle> # \<kappa>\<rangle>
+"
+ apply (rule accept_state.Any)
+    apply (erule flow_state_to_flow_exp_5, simp, auto)
+   apply (erule flow_state_to_flow_env_5, simp, auto)
+  apply (erule flow_state_to_flow_stack_5, simp, auto)
+done
+
+
+lemma flow_state_to_flow_exp_6: "
+  (\<G>, \<V>) \<Turnstile>\<^sub>\<sigma>  \<langle>LET x = FST x\<^sub>p in e; \<rho>; \<kappa>\<rangle> \<Longrightarrow> \<rho> x\<^sub>p = Some \<lbrace>prim.Pair x\<^sub>1 x\<^sub>2, \<rho>\<^sub>p\<rbrace> \<Longrightarrow> 
+  \<rho>\<^sub>p x\<^sub>1 = Some \<omega> \<Longrightarrow> (\<G>, \<V>) \<Turnstile>\<^sub>e  e
+"
+ apply (erule accept_state.cases, auto)
+ apply (erule accept_exp.cases, auto)
+done
+
+lemma flow_state_to_flow_env_6: "
+  (\<G>, \<V>) \<Turnstile>\<^sub>\<sigma>  \<langle>LET x = FST x\<^sub>p in e; \<rho>; \<kappa>\<rangle> \<Longrightarrow> \<rho> x\<^sub>p = Some \<lbrace>prim.Pair x\<^sub>1 x\<^sub>2, \<rho>\<^sub>p\<rbrace> \<Longrightarrow> \<rho>\<^sub>p x\<^sub>1 = Some \<omega> \<Longrightarrow> (\<G>, \<V>) \<Turnstile>\<^sub>\<rho> \<rho>(x \<mapsto> \<omega>)
+"
+ apply (rule accept_value_accept_val_env.Any, auto)
+      apply (erule accept_state.cases, auto)
+      apply (erule accept_val_env.cases, auto)
+      apply (drule spec[of _ x\<^sub>p]; auto)
+      apply (erule accept_value.cases, auto)
+      apply (erule accept_val_env.cases, auto)
+      apply (drule spec[of _ x\<^sub>1]; auto)
+      apply (erule accept_exp.cases, auto)
+     apply (erule accept_state.cases, auto)
+     apply (erule accept_val_env.cases, auto)
+     apply (drule spec[of _ x\<^sub>p]; auto)
+     apply (erule accept_value.cases, auto)
+     apply (erule accept_val_env.cases, auto)
+    apply (rename_tac x' \<omega>')
+    apply (erule accept_state.cases, auto)
+    apply (erule accept_val_env.cases, auto)
+   apply (rename_tac x' \<omega>')
+   apply (erule accept_state.cases, auto)
+   apply (erule accept_val_env.cases, auto)
+done
+
+lemma flow_state_to_flow_stack_6: "
+  (\<G>, \<V>) \<Turnstile>\<^sub>\<sigma>  \<langle>LET x = FST x\<^sub>p in e; \<rho>; \<kappa>\<rangle> \<Longrightarrow> \<rho> x\<^sub>p = Some \<lbrace>prim.Pair x\<^sub>1 x\<^sub>2, \<rho>\<^sub>p\<rbrace> \<Longrightarrow> \<rho>\<^sub>p x\<^sub>1 = Some \<omega> \<Longrightarrow> (\<G>, \<V>) \<Turnstile>\<^sub>\<kappa>  \<V> (\<lfloor>e\<rfloor>) \<Rrightarrow> \<kappa>
+"
+ apply (erule accept_state.cases, auto)
+done
+
+lemma flow_over_state_6: "
+  (\<G>, \<V>) \<Turnstile>\<^sub>\<sigma>  \<langle>LET x = FST x\<^sub>p in e; \<rho>; \<kappa>\<rangle> \<Longrightarrow>
+  \<rho> x\<^sub>p = Some \<lbrace>prim.Pair x\<^sub>1 x\<^sub>2, \<rho>\<^sub>p\<rbrace> \<Longrightarrow> \<rho>\<^sub>p x\<^sub>1 = Some \<omega> \<Longrightarrow> 
+  (\<G>, \<V>) \<Turnstile>\<^sub>\<sigma>  \<langle>e; \<rho>(x \<mapsto> \<omega>); \<kappa>\<rangle>
+"
+ apply (rule accept_state.Any)
+    apply (erule flow_state_to_flow_exp_6, simp, auto)
+   apply (erule flow_state_to_flow_env_6, simp, auto)
+  apply (erule flow_state_to_flow_stack_6, simp, auto)
+done
+
+lemma flow_state_to_flow_exp_7: "
+  (\<G>, \<V>) \<Turnstile>\<^sub>\<sigma>  \<langle>LET x = SND x\<^sub>p in e; \<rho>; \<kappa>\<rangle> \<Longrightarrow> \<rho> x\<^sub>p = Some \<lbrace>prim.Pair x\<^sub>1 x\<^sub>2, \<rho>\<^sub>p\<rbrace> \<Longrightarrow> 
+  \<rho>\<^sub>p x\<^sub>2 = Some \<omega> \<Longrightarrow> (\<G>, \<V>) \<Turnstile>\<^sub>e  e
+"
+ apply (erule accept_state.cases, auto)
+ apply (erule accept_exp.cases, auto)
+done
+
+lemma flow_state_to_flow_env_7: "
+  (\<G>, \<V>) \<Turnstile>\<^sub>\<sigma>  \<langle>LET x = SND x\<^sub>p in e; \<rho>; \<kappa>\<rangle> \<Longrightarrow> \<rho> x\<^sub>p = Some \<lbrace>prim.Pair x\<^sub>1 x\<^sub>2, \<rho>\<^sub>p\<rbrace> \<Longrightarrow> \<rho>\<^sub>p x\<^sub>2 = Some \<omega> \<Longrightarrow> (\<G>, \<V>) \<Turnstile>\<^sub>\<rho> \<rho>(x \<mapsto> \<omega>)
+"
+ apply (rule accept_value_accept_val_env.Any, auto)
+      apply (erule accept_state.cases, auto)
+      apply (erule accept_val_env.cases, auto)
+      apply (drule spec[of _ x\<^sub>p]; auto)
+      apply (erule accept_value.cases, auto)
+      apply (erule accept_val_env.cases, auto)
+      apply (drule spec[of _ x\<^sub>2]; auto)
+      apply (erule accept_exp.cases, auto)
+     apply (erule accept_state.cases, auto)
+     apply (erule accept_val_env.cases, auto)
+     apply (drule spec[of _ x\<^sub>p]; auto)
+     apply (erule accept_value.cases, auto)
+     apply (erule accept_val_env.cases, auto)
+    apply (rename_tac x' \<omega>')
+    apply (erule accept_state.cases, auto)
+    apply (erule accept_val_env.cases, auto)
+   apply (rename_tac x' \<omega>')
+   apply (erule accept_state.cases, auto)
+   apply (erule accept_val_env.cases, auto)
+done
+
+lemma flow_state_to_flow_stack_7: "
+  (\<G>, \<V>) \<Turnstile>\<^sub>\<sigma>  \<langle>LET x = SND x\<^sub>p in e; \<rho>; \<kappa>\<rangle> \<Longrightarrow> \<rho> x\<^sub>p = Some \<lbrace>prim.Pair x\<^sub>1 x\<^sub>2, \<rho>\<^sub>p\<rbrace> \<Longrightarrow> \<rho>\<^sub>p x\<^sub>2 = Some \<omega> \<Longrightarrow> (\<G>, \<V>) \<Turnstile>\<^sub>\<kappa>  \<V> (\<lfloor>e\<rfloor>) \<Rrightarrow> \<kappa>
+"
+ apply (erule accept_state.cases, auto)
+done
+
+lemma flow_over_state_7: "
+  (\<G>, \<V>) \<Turnstile>\<^sub>\<sigma>  \<langle>LET x = SND x\<^sub>p in e; \<rho>; \<kappa>\<rangle> \<Longrightarrow>
+  \<rho> x\<^sub>p = Some \<lbrace>prim.Pair x\<^sub>1 x\<^sub>2, \<rho>\<^sub>p\<rbrace> \<Longrightarrow> \<rho>\<^sub>p x\<^sub>2 = Some \<omega> \<Longrightarrow> 
+  (\<G>, \<V>) \<Turnstile>\<^sub>\<sigma>  \<langle>e; \<rho>(x \<mapsto> \<omega>); \<kappa>\<rangle>
+"
+ apply (rule accept_state.Any)
+    apply (erule flow_state_to_flow_exp_7, simp, auto)
+   apply (erule flow_state_to_flow_env_7, simp, auto)
+  apply (erule flow_state_to_flow_stack_7, simp, auto)
+done
+
+lemma flow_state_to_flow_exp_8: "
+ (\<G>, \<V>) \<Turnstile>\<^sub>\<sigma>  \<langle>LET x = APP f x\<^sub>a in e; \<rho>; \<kappa>\<rangle> \<Longrightarrow> 
+ \<rho> f = Some \<lbrace>Abs f\<^sub>l x\<^sub>l e\<^sub>l, \<rho>\<^sub>l\<rbrace> \<Longrightarrow> \<rho> x\<^sub>a = Some \<omega>\<^sub>a \<Longrightarrow> 
+ (\<G>, \<V>) \<Turnstile>\<^sub>e  e\<^sub>l
+"
+ apply (erule accept_state.cases, auto)
+ apply (erule accept_exp.cases, auto)
+ apply (erule accept_val_env.cases, auto)
+ apply (drule spec[of _ f]; auto)
+ apply (erule accept_value.cases, auto)
+done
+
+lemma flow_state_to_flow_env_8: "
+  (\<G>, \<V>) \<Turnstile>\<^sub>\<sigma>  \<langle>LET x = APP f x\<^sub>a in e; \<rho>; \<kappa>\<rangle> \<Longrightarrow> 
+  \<rho> f = Some \<lbrace>Abs f\<^sub>l x\<^sub>l e\<^sub>l, \<rho>\<^sub>l\<rbrace> \<Longrightarrow> \<rho> x\<^sub>a = Some \<omega>\<^sub>a \<Longrightarrow> 
+  (\<G>, \<V>) \<Turnstile>\<^sub>\<rho> \<rho>\<^sub>l(f\<^sub>l \<mapsto> \<lbrace>Abs f\<^sub>l x\<^sub>l e\<^sub>l, \<rho>\<^sub>l\<rbrace>, x\<^sub>l \<mapsto> \<omega>\<^sub>a)
+"
+ apply (rule accept_value_accept_val_env.Any, auto)
+           apply (erule accept_state.cases, auto)
+           apply (erule accept_exp.cases, auto, (drule spec)+, auto)
+            apply (erule accept_val_env.cases, auto, (drule spec)+, auto)
+           apply (erule accept_val_env.cases, auto)
+          apply (erule accept_state.cases, auto)
+          apply (erule accept_val_env.cases, auto)
+         apply (erule accept_state.cases, auto)
+         apply (erule accept_val_env.cases, auto)
+         apply (drule spec[of _ f]; auto)
+         apply (erule accept_value.cases, auto)
+        apply (erule accept_state.cases, auto)
+        apply (erule accept_val_env.cases, auto)
+       apply (erule accept_state.cases, auto)
+       apply (erule accept_val_env.cases, auto)
+       apply (frule spec[of _ f])
+       apply (drule spec[of _ "\<lbrace>Abs f\<^sub>l x\<^sub>l e\<^sub>l, \<rho>\<^sub>l\<rbrace>"])
+       apply (drule spec[of _ x\<^sub>a])
+       apply (drule spec[of _ \<omega>\<^sub>a], auto)
+       apply (erule accept_exp.cases, auto)
+      apply (erule accept_state.cases, auto)
+      apply (erule accept_val_env.cases, auto)
+     apply (rename_tac x' \<omega>)
+     apply (erule accept_state.cases, auto)
+     apply (erule accept_val_env.cases, auto)
+     apply (frule spec[of _ f])
+     apply (drule spec[of _ "\<lbrace>Abs f\<^sub>l x\<^sub>l e\<^sub>l, \<rho>\<^sub>l\<rbrace>"])
+     apply (drule spec[of _ x\<^sub>a])
+     apply (drule spec[of _ \<omega>\<^sub>a]; auto)
+     apply (erule accept_value.cases, auto)
+     apply (erule accept_val_env.cases, auto)
+    apply (rename_tac x' \<omega>)
+    apply (erule accept_state.cases, auto)
+    apply (erule accept_val_env.cases, auto)
+    apply (frule spec[of _ f])
+    apply (drule spec[of _ "\<lbrace>Abs f\<^sub>l x\<^sub>l e\<^sub>l, \<rho>\<^sub>l\<rbrace>"])
+    apply (drule spec[of _ x\<^sub>a])
+    apply (drule spec[of _ \<omega>\<^sub>a]; auto)
+    apply (erule accept_value.cases, auto)
+    apply (erule accept_val_env.cases, auto)
+done
+
+lemma flow_state_to_flow_stack_8: "
+  (\<G>, \<V>) \<Turnstile>\<^sub>\<sigma>  \<langle>LET x = APP f x\<^sub>a in e; \<rho>; \<kappa>\<rangle> \<Longrightarrow> 
+  \<rho> f = Some \<lbrace>Abs f\<^sub>l x\<^sub>l e\<^sub>l, \<rho>\<^sub>l\<rbrace> \<Longrightarrow> \<rho> x\<^sub>a = Some \<omega>\<^sub>a \<Longrightarrow> 
+  (\<G>, \<V>) \<Turnstile>\<^sub>\<kappa>  \<V> (\<lfloor>e\<^sub>l\<rfloor>) \<Rrightarrow> \<langle>x,e,\<rho>\<rangle> # \<kappa>
+"
+ apply (rule accept_stack.Nonempty)
+    apply (erule accept_state.cases, auto) 
+    apply (erule accept_exp.cases, auto)
+    apply (erule accept_val_env.cases, (drule spec)+, auto)
+   apply (erule accept_state.cases, auto) 
+   apply (erule accept_exp.cases, auto)
+  apply (erule accept_state.cases, auto) 
+ apply (erule accept_state.cases, auto) 
+done
+
+lemma flow_over_state_8: "
+  (\<G>, \<V>) \<Turnstile>\<^sub>\<sigma>  \<langle>LET x = APP f x\<^sub>a in e; \<rho>; \<kappa>\<rangle> \<Longrightarrow>
+  \<rho> f = Some \<lbrace>Abs f\<^sub>l x\<^sub>l e\<^sub>l, \<rho>\<^sub>l\<rbrace> \<Longrightarrow> \<rho> x\<^sub>a = Some \<omega>\<^sub>a \<Longrightarrow> 
+  (\<G>, \<V>) \<Turnstile>\<^sub>\<sigma>  \<langle>e\<^sub>l; \<rho>\<^sub>l(f\<^sub>l \<mapsto> \<lbrace>Abs f\<^sub>l x\<^sub>l e\<^sub>l, \<rho>\<^sub>l\<rbrace>, x\<^sub>l \<mapsto> \<omega>\<^sub>a); \<langle>x,e,\<rho>\<rangle> # \<kappa>\<rangle>
+"
+ apply (rule accept_state.Any)
+    apply (erule flow_state_to_flow_exp_8, simp, auto)
+   apply (erule flow_state_to_flow_env_8, simp, auto)
+  apply (erule flow_state_to_flow_stack_8, simp, auto)
+done
+*)
+
+theorem flow_over_state_preservation : "
+  \<lbrakk>
+    (\<G>, \<V>) \<Turnstile>\<^sub>\<sigma> \<sigma>; 
+    \<sigma> \<hookrightarrow> \<sigma>'
+  \<rbrakk> \<Longrightarrow>
+  (\<G>, \<V>) \<Turnstile>\<^sub>\<sigma> \<sigma>'
+"
+ apply (erule seq_step.cases, auto)
+        apply (erule flow_over_state_1, auto)
+       apply (erule flow_over_state_2)
+      apply (erule flow_over_state_3)
+     apply (erule flow_over_state_4, simp, auto)
+    apply (erule flow_over_state_5, simp, auto)
+   apply (erule flow_over_state_6, simp, auto)
+  apply (erule flow_over_state_7, simp, auto)
+ apply (erule flow_over_state_8, auto)
+sorry
+
+lemma flow_seq_step_preservation: "
+  (\<G>, \<V>) \<Turnstile>\<^sub>\<E> \<E> \<Longrightarrow> leaf \<E> \<pi> \<Longrightarrow> \<E> \<pi> = Some (\<langle>LET x = b in e; \<rho>; \<kappa>\<rangle>) \<Longrightarrow> 
+  \<langle>LET x = b in e; \<rho>; \<kappa>\<rangle> \<hookrightarrow> \<sigma>' \<Longrightarrow> (\<G>, \<V>) \<Turnstile>\<^sub>\<E> \<E>(\<pi> ;; x \<mapsto> \<sigma>')
+"
+ apply (rule accept_state_pool.Any, auto)
+  apply (erule accept_state_pool.cases, auto)
+  apply ((drule spec)+, auto)
+  apply (erule flow_over_state_preservation, auto)
+ apply (erule accept_state_pool.cases, auto)
+done
+
+(*
+lemma flow_over_pool_to_exp_1: "
+  (\<G>, \<V>) \<Turnstile>\<^sub>\<E> \<E> \<Longrightarrow>
+  \<E> \<pi>\<^sub>s = Some (\<langle>LET x\<^sub>s = SYNC x\<^sub>s\<^sub>e in e\<^sub>s; \<rho>\<^sub>s; \<kappa>\<^sub>s\<rangle>) \<Longrightarrow>
+  (\<G>, \<V>) \<Turnstile>\<^sub>e e\<^sub>s
+"
+ apply (erule accept_state_pool.cases, auto)
+ apply (drule spec[of _ \<pi>\<^sub>s])
+ apply (drule spec[of _ "\<langle>LET x\<^sub>s = SYNC x\<^sub>s\<^sub>e in e\<^sub>s; \<rho>\<^sub>s; \<kappa>\<^sub>s\<rangle>"], auto)
+ apply (erule accept_state.cases, auto)
+ apply (erule accept_exp.cases, auto)
+done
+
+lemma flow_over_pool_to_env_1: "
+  (\<G>, \<V>) \<Turnstile>\<^sub>\<E> \<E> \<Longrightarrow>
+  \<E> \<pi>\<^sub>s = Some (\<langle>LET x\<^sub>s = SYNC x\<^sub>s\<^sub>e in e\<^sub>s; \<rho>\<^sub>s; \<kappa>\<^sub>s\<rangle>) \<Longrightarrow>
+  \<rho>\<^sub>s x\<^sub>s\<^sub>e = Some \<lbrace>Send_Evt x\<^sub>s\<^sub>c x\<^sub>m, \<rho>\<^sub>s\<^sub>e\<rbrace> \<Longrightarrow>
+  \<rho>\<^sub>s\<^sub>e x\<^sub>s\<^sub>c = Some \<lbrace>c\<rbrace> \<Longrightarrow>
+  \<E> \<pi>\<^sub>r = Some (\<langle>LET x\<^sub>r = SYNC x\<^sub>r\<^sub>e in e\<^sub>r; \<rho>\<^sub>r; \<kappa>\<^sub>r\<rangle>) \<Longrightarrow>
+  \<rho>\<^sub>r x\<^sub>r\<^sub>e = Some \<lbrace>Recv_Evt x\<^sub>r\<^sub>c, \<rho>\<^sub>r\<^sub>e\<rbrace> \<Longrightarrow>
+  \<rho>\<^sub>r\<^sub>e x\<^sub>r\<^sub>c = Some \<lbrace>c\<rbrace> \<Longrightarrow>
+  (\<G>, \<V>) \<Turnstile>\<^sub>\<rho> \<rho>\<^sub>s(x\<^sub>s \<mapsto> \<lbrace>\<rbrace>)
+"
+apply (rule accept_value_accept_val_env.Any; auto)
+    apply (erule accept_state_pool.cases, auto)
+    apply (frule spec[of _ \<pi>\<^sub>s])
+    apply (drule spec[of _ \<pi>\<^sub>r])
+    apply (drule spec[of _ "\<langle>LET x\<^sub>s = SYNC x\<^sub>s\<^sub>e in e\<^sub>s; \<rho>\<^sub>s; \<kappa>\<^sub>s\<rangle>"])
+    apply (drule spec[of _ "\<langle>LET x\<^sub>r = SYNC x\<^sub>r\<^sub>e in e\<^sub>r; \<rho>\<^sub>r; \<kappa>\<^sub>r\<rangle>"])
+    apply (drule mp[of "\<E> \<pi>\<^sub>s = Some (\<langle>LET x\<^sub>s = SYNC x\<^sub>s\<^sub>e in e\<^sub>s; \<rho>\<^sub>s; \<kappa>\<^sub>s\<rangle>) "])
+    apply (drule mp[of "\<E> \<pi>\<^sub>r = Some (\<langle>LET x\<^sub>r = SYNC x\<^sub>r\<^sub>e in e\<^sub>r; \<rho>\<^sub>r; \<kappa>\<^sub>r\<rangle>)"], auto)
+    apply (erule accept_state.cases[of "(\<G>, \<V>)" "\<langle>LET x\<^sub>r = SYNC x\<^sub>r\<^sub>e in e\<^sub>r; \<rho>\<^sub>r; \<kappa>\<^sub>r\<rangle>"], auto)
+    apply (erule accept_state.cases[of "(\<G>, \<V>)" "\<langle>LET x\<^sub>s = SYNC x\<^sub>s\<^sub>e in e\<^sub>s; \<rho>\<^sub>s; \<kappa>\<^sub>s\<rangle>"], auto)
+    apply (erule accept_val_env.cases[of "(\<G>, \<V>)" "\<rho>\<^sub>r"], auto)
+    apply (erule accept_val_env.cases[of "(\<G>, \<V>)" "\<rho>\<^sub>s"], auto)
+    apply (drule spec[of _ x\<^sub>r\<^sub>e])
+    apply (drule spec[of _ x\<^sub>s\<^sub>e])
+    apply (drule spec[of _ "\<lbrace>Recv_Evt x\<^sub>r\<^sub>c, \<rho>\<^sub>r\<^sub>e\<rbrace>"])
+    apply (drule spec[of _ "\<lbrace>Send_Evt x\<^sub>s\<^sub>c x\<^sub>m, \<rho>\<^sub>s\<^sub>e\<rbrace>"])
+    apply (drule mp[of "\<rho>\<^sub>r x\<^sub>r\<^sub>e = Some \<lbrace>Recv_Evt x\<^sub>r\<^sub>c, \<rho>\<^sub>r\<^sub>e\<rbrace>"], simp)
+    apply (drule mp[of "\<rho>\<^sub>s x\<^sub>s\<^sub>e = Some \<lbrace>Send_Evt x\<^sub>s\<^sub>c x\<^sub>m, \<rho>\<^sub>s\<^sub>e\<rbrace>"]; auto)
+    apply (erule accept_value.cases[of "(\<G>, \<V>)" "\<lbrace>Recv_Evt x\<^sub>r\<^sub>c, \<rho>\<^sub>r\<^sub>e\<rbrace>"]; auto)
+    apply (erule accept_value.cases[of "(\<G>, \<V>)" "\<lbrace>Send_Evt x\<^sub>s\<^sub>c x\<^sub>m, \<rho>\<^sub>s\<^sub>e\<rbrace> "]; auto)
+    apply (erule accept_val_env.cases[of "(\<G>, \<V>)" "\<rho>\<^sub>r\<^sub>e"], auto)
+    apply (erule accept_val_env.cases[of "(\<G>, \<V>)" "\<rho>\<^sub>s\<^sub>e"], auto)
+    apply (erule accept_exp.cases[of "(\<G>, \<V>)" "LET x\<^sub>r = SYNC x\<^sub>r\<^sub>e in e\<^sub>r"]; auto)
+    apply (erule accept_exp.cases[of "(\<G>, \<V>)" "LET x\<^sub>s = SYNC x\<^sub>s\<^sub>e in e\<^sub>s"]; auto)
+    apply (thin_tac "\<forall>x\<^sub>s\<^sub>c x\<^sub>m. ^Send_Evt x\<^sub>s\<^sub>c x\<^sub>m \<in> \<V> x\<^sub>r\<^sub>e \<longrightarrow> (\<forall>x\<^sub>c. ^Chan x\<^sub>c \<in> \<V> x\<^sub>s\<^sub>c \<longrightarrow> ^\<lparr>\<rparr> \<in> \<V> x\<^sub>r \<and> \<V> x\<^sub>m \<subseteq> \<C> x\<^sub>c)")
+    apply (thin_tac "\<forall>x\<^sub>r\<^sub>c. ^Recv_Evt x\<^sub>r\<^sub>c \<in> \<V> x\<^sub>s\<^sub>e \<longrightarrow> (\<forall>x\<^sub>c. ^Chan x\<^sub>c \<in> \<V> x\<^sub>r\<^sub>c \<longrightarrow> \<C> x\<^sub>c \<subseteq> \<V> x\<^sub>s)")
+    apply (drule spec[of _ x\<^sub>r\<^sub>c])
+    apply (drule spec[of _ x\<^sub>s\<^sub>c])
+    apply (drule spec[of _ x\<^sub>r\<^sub>c])
+    apply (drule spec[of _ x\<^sub>s\<^sub>c])
+    apply (case_tac c; auto)
+    apply (rule accept_value_accept_val_env.Unit)
+   apply (erule accept_state_pool.cases, auto)
+   apply (drule spec[of _ \<pi>\<^sub>s])
+   apply (drule spec[of _ "\<langle>LET x\<^sub>s = SYNC x\<^sub>s\<^sub>e in e\<^sub>s; \<rho>\<^sub>s; \<kappa>\<^sub>s\<rangle>"]; auto)
+   apply (erule accept_state.cases; auto)
+   apply (drule accept_val_env.cases; auto)
+  apply (erule accept_state_pool.cases, auto)
+  apply (drule spec[of _ \<pi>\<^sub>s])
+  apply (drule spec[of _ "\<langle>LET x\<^sub>s = SYNC x\<^sub>s\<^sub>e in e\<^sub>s; \<rho>\<^sub>s; \<kappa>\<^sub>s\<rangle>"]; auto)
+  apply (erule accept_state.cases; auto)
+  apply (drule accept_val_env.cases; auto)
+done
+
+lemma flow_over_pool_to_stack_1: "
+  (\<G>, \<V>) \<Turnstile>\<^sub>\<E> \<E> \<Longrightarrow>
+  \<E> \<pi>\<^sub>s = Some (\<langle>LET x\<^sub>s = SYNC x\<^sub>s\<^sub>e in e\<^sub>s; \<rho>\<^sub>s; \<kappa>\<^sub>s\<rangle>) \<Longrightarrow>
+  (\<G>, \<V>) \<Turnstile>\<^sub>\<kappa>  \<V> (\<lfloor>e\<^sub>s\<rfloor>) \<Rrightarrow> \<kappa>\<^sub>s
+"
+ apply (erule accept_state_pool.cases, auto)
+ apply (drule spec[of _ \<pi>\<^sub>s])
+ apply (drule spec[of _ "\<langle>LET x\<^sub>s = SYNC x\<^sub>s\<^sub>e in e\<^sub>s; \<rho>\<^sub>s; \<kappa>\<^sub>s\<rangle>"], auto)
+ apply (erule accept_state.cases, auto) 
+done
+
+lemma flow_over_pool_to_exp_2: "
+  (\<G>, \<V>) \<Turnstile>\<^sub>\<E> \<E> \<Longrightarrow>
+  \<E> \<pi>\<^sub>r = Some (\<langle>LET x\<^sub>r = SYNC x\<^sub>r\<^sub>e in e\<^sub>r; \<rho>\<^sub>r; \<kappa>\<^sub>r\<rangle>) \<Longrightarrow> 
+  (\<G>, \<V>) \<Turnstile>\<^sub>e  e\<^sub>r
+"
+ apply (erule accept_state_pool.cases, auto)
+ apply (drule spec[of _ \<pi>\<^sub>r])
+ apply (drule spec[of _ "\<langle>LET x\<^sub>r = SYNC x\<^sub>r\<^sub>e in e\<^sub>r; \<rho>\<^sub>r; \<kappa>\<^sub>r\<rangle>"], auto)
+ apply (erule accept_state.cases, auto)
+ apply (erule accept_exp.cases, auto)
+done
+
+lemma flow_over_pool_to_env_2: "
+  (\<G>, \<V>) \<Turnstile>\<^sub>\<E> \<E> \<Longrightarrow>
+  \<E>' = \<E>(\<pi>\<^sub>s ;; x\<^sub>s \<mapsto> \<langle>e\<^sub>s; \<rho>\<^sub>s(x\<^sub>s \<mapsto> \<lbrace>\<rbrace>); \<kappa>\<^sub>s\<rangle>, \<pi>\<^sub>r ;; x\<^sub>r \<mapsto> \<langle>e\<^sub>r; \<rho>\<^sub>r(x\<^sub>r \<mapsto> \<omega>\<^sub>m); \<kappa>\<^sub>r\<rangle>) \<Longrightarrow>
+  leaf \<E> \<pi>\<^sub>s \<Longrightarrow>
+  \<E> \<pi>\<^sub>s = Some (\<langle>LET x\<^sub>s = SYNC x\<^sub>s\<^sub>e in e\<^sub>s; \<rho>\<^sub>s; \<kappa>\<^sub>s\<rangle>) \<Longrightarrow>
+  \<rho>\<^sub>s x\<^sub>s\<^sub>e = Some \<lbrace>Send_Evt x\<^sub>s\<^sub>c x\<^sub>m, \<rho>\<^sub>s\<^sub>e\<rbrace> \<Longrightarrow>
+  \<rho>\<^sub>s\<^sub>e x\<^sub>s\<^sub>c = Some \<lbrace>c\<rbrace> \<Longrightarrow>
+  \<rho>\<^sub>s\<^sub>e x\<^sub>m = Some \<omega>\<^sub>m \<Longrightarrow>
+  leaf \<E> \<pi>\<^sub>r \<Longrightarrow>
+  \<E> \<pi>\<^sub>r = Some (\<langle>LET x\<^sub>r = SYNC x\<^sub>r\<^sub>e in e\<^sub>r; \<rho>\<^sub>r; \<kappa>\<^sub>r\<rangle>) \<Longrightarrow> 
+  \<rho>\<^sub>r x\<^sub>r\<^sub>e = Some \<lbrace>Recv_Evt x\<^sub>r\<^sub>c, \<rho>\<^sub>r\<^sub>e\<rbrace> \<Longrightarrow> 
+  \<rho>\<^sub>r\<^sub>e x\<^sub>r\<^sub>c = Some \<lbrace>c\<rbrace> \<Longrightarrow> 
+  (\<G>, \<V>) \<Turnstile>\<^sub>\<rho> \<rho>\<^sub>r(x\<^sub>r \<mapsto> \<omega>\<^sub>m)
+"
+apply (rule accept_value_accept_val_env.Any; auto)
+      apply (erule accept_state_pool.cases, auto)
+      apply (frule spec[of _ \<pi>\<^sub>s])
+      apply (drule spec[of _ \<pi>\<^sub>r])
+      apply (drule spec[of _ "\<langle>LET x\<^sub>s = SYNC x\<^sub>s\<^sub>e in e\<^sub>s; \<rho>\<^sub>s; \<kappa>\<^sub>s\<rangle>"])
+      apply (drule spec[of _ "\<langle>LET x\<^sub>r = SYNC x\<^sub>r\<^sub>e in e\<^sub>r; \<rho>\<^sub>r; \<kappa>\<^sub>r\<rangle>"])
+      apply (drule mp[of "\<E> \<pi>\<^sub>s = Some (\<langle>LET x\<^sub>s = SYNC x\<^sub>s\<^sub>e in e\<^sub>s; \<rho>\<^sub>s; \<kappa>\<^sub>s\<rangle>) "])
+      apply (drule mp[of "\<E> \<pi>\<^sub>r = Some (\<langle>LET x\<^sub>r = SYNC x\<^sub>r\<^sub>e in e\<^sub>r; \<rho>\<^sub>r; \<kappa>\<^sub>r\<rangle>)"], auto)
+      apply (erule accept_state.cases[of "(\<G>, \<V>)" "\<langle>LET x\<^sub>r = SYNC x\<^sub>r\<^sub>e in e\<^sub>r; \<rho>\<^sub>r; \<kappa>\<^sub>r\<rangle>"], auto)
+      apply (erule accept_state.cases[of "(\<G>, \<V>)" "\<langle>LET x\<^sub>s = SYNC x\<^sub>s\<^sub>e in e\<^sub>s; \<rho>\<^sub>s; \<kappa>\<^sub>s\<rangle>"], auto)
+      apply (erule accept_val_env.cases[of "(\<G>, \<V>)" "\<rho>\<^sub>r"], auto)
+      apply (erule accept_val_env.cases[of "(\<G>, \<V>)" "\<rho>\<^sub>s"], auto)
+      apply (drule spec[of _ x\<^sub>r\<^sub>e])
+      apply (drule spec[of _ x\<^sub>s\<^sub>e])
+      apply (drule spec[of _ "\<lbrace>Recv_Evt x\<^sub>r\<^sub>c, \<rho>\<^sub>r\<^sub>e\<rbrace>"])
+      apply (drule spec[of _ "\<lbrace>Send_Evt x\<^sub>s\<^sub>c x\<^sub>m, \<rho>\<^sub>s\<^sub>e\<rbrace>"])
+      apply (drule mp[of "\<rho>\<^sub>r x\<^sub>r\<^sub>e = Some \<lbrace>Recv_Evt x\<^sub>r\<^sub>c, \<rho>\<^sub>r\<^sub>e\<rbrace>"], simp)
+      apply (drule mp[of "\<rho>\<^sub>s x\<^sub>s\<^sub>e = Some \<lbrace>Send_Evt x\<^sub>s\<^sub>c x\<^sub>m, \<rho>\<^sub>s\<^sub>e\<rbrace>"]; auto)
+      apply (erule accept_value.cases[of "(\<G>, \<V>)" "\<lbrace>Recv_Evt x\<^sub>r\<^sub>c, \<rho>\<^sub>r\<^sub>e\<rbrace>"]; auto)
+      apply (erule accept_value.cases[of "(\<G>, \<V>)" "\<lbrace>Send_Evt x\<^sub>s\<^sub>c x\<^sub>m, \<rho>\<^sub>s\<^sub>e\<rbrace> "]; auto)
+      apply (erule accept_val_env.cases[of "(\<G>, \<V>)" "\<rho>\<^sub>r\<^sub>e"], auto)
+      apply (erule accept_val_env.cases[of "(\<G>, \<V>)" "\<rho>\<^sub>s\<^sub>e"], auto)
+      apply (erule accept_exp.cases[of "(\<G>, \<V>)" "LET x\<^sub>r = SYNC x\<^sub>r\<^sub>e in e\<^sub>r"]; auto)
+      apply (erule accept_exp.cases[of "(\<G>, \<V>)" "LET x\<^sub>s = SYNC x\<^sub>s\<^sub>e in e\<^sub>s"]; auto)
+      apply (thin_tac "\<forall>x\<^sub>s\<^sub>c x\<^sub>m. ^Send_Evt x\<^sub>s\<^sub>c x\<^sub>m \<in> \<V> x\<^sub>r\<^sub>e \<longrightarrow> (\<forall>x\<^sub>c. ^Chan x\<^sub>c \<in> \<V> x\<^sub>s\<^sub>c \<longrightarrow> ^\<lparr>\<rparr> \<in> \<V> x\<^sub>r \<and> \<V> x\<^sub>m \<subseteq> \<C> x\<^sub>c)")
+      apply (thin_tac "\<forall>x\<^sub>r\<^sub>c. ^Recv_Evt x\<^sub>r\<^sub>c \<in> \<V> x\<^sub>s\<^sub>e \<longrightarrow> (\<forall>x\<^sub>c. ^Chan x\<^sub>c \<in> \<V> x\<^sub>r\<^sub>c \<longrightarrow> \<C> x\<^sub>c \<subseteq> \<V> x\<^sub>s)")
+      apply (drule spec[of _ x\<^sub>r\<^sub>c])
+      apply (frule spec[of _ x\<^sub>s\<^sub>c])
+      apply (drule spec[of _ x\<^sub>m])
+      apply (drule spec[of _ x\<^sub>r\<^sub>c])
+      apply (drule spec[of _ x\<^sub>s\<^sub>c])
+      apply (drule spec[of _ "\<lbrace>c\<rbrace>"])
+      apply (drule spec[of _ "\<lbrace>c\<rbrace>"])
+      apply (drule spec[of _ "\<omega>\<^sub>m"])
+      apply (drule spec[of _ "x\<^sub>m"])
+      apply (case_tac c, rename_tac \<pi> x\<^sub>c, auto)
+
+    apply (erule accept_state_pool.cases, auto)
+    apply (drule spec[of _ \<pi>\<^sub>s])
+    apply (drule spec[of _ "\<langle>LET x\<^sub>s = SYNC x\<^sub>s\<^sub>e in e\<^sub>s; \<rho>\<^sub>s; \<kappa>\<^sub>s\<rangle>"])
+    apply (drule mp[of "\<E> \<pi>\<^sub>s = Some (\<langle>LET x\<^sub>s = SYNC x\<^sub>s\<^sub>e in e\<^sub>s; \<rho>\<^sub>s; \<kappa>\<^sub>s\<rangle>) "], auto)
+    apply (erule accept_state.cases[of "(\<G>, \<V>)" "\<langle>LET x\<^sub>s = SYNC x\<^sub>s\<^sub>e in e\<^sub>s; \<rho>\<^sub>s; \<kappa>\<^sub>s\<rangle>"], auto)
+    apply (erule accept_val_env.cases[of "(\<G>, \<V>)" "\<rho>\<^sub>s"], auto)
+    apply (drule spec[of _ x\<^sub>s\<^sub>e])
+    apply (drule spec[of _ "\<lbrace>Send_Evt x\<^sub>s\<^sub>c x\<^sub>m, \<rho>\<^sub>s\<^sub>e\<rbrace>"])
+    apply (drule mp[of "\<rho>\<^sub>s x\<^sub>s\<^sub>e = Some \<lbrace>Send_Evt x\<^sub>s\<^sub>c x\<^sub>m, \<rho>\<^sub>s\<^sub>e\<rbrace>"]; auto)
+    apply (erule accept_value.cases[of "(\<G>, \<V>)" "\<lbrace>Send_Evt x\<^sub>s\<^sub>c x\<^sub>m, \<rho>\<^sub>s\<^sub>e\<rbrace> "]; auto)
+    apply (erule accept_val_env.cases[of "(\<G>, \<V>)" "\<rho>\<^sub>s\<^sub>e"], auto)
+   apply (erule accept_state_pool.cases, auto)
+   apply (drule spec[of _ \<pi>\<^sub>r])
+   apply (drule spec[of _ "\<langle>LET x\<^sub>r = SYNC x\<^sub>r\<^sub>e in e\<^sub>r; \<rho>\<^sub>r; \<kappa>\<^sub>r\<rangle>"]; auto)
+   apply (erule accept_state.cases; auto)
+   apply (drule accept_val_env.cases; auto)
+  apply (erule accept_state_pool.cases, auto)
+  apply (drule spec[of _ \<pi>\<^sub>r])
+  apply (drule spec[of _ "\<langle>LET x\<^sub>r = SYNC x\<^sub>r\<^sub>e in e\<^sub>r; \<rho>\<^sub>r; \<kappa>\<^sub>r\<rangle>"]; auto)
+  apply (erule accept_state.cases; auto)
+  apply (drule accept_val_env.cases; auto)
+done
+
+lemma flow_over_pool_to_stack_2: "
+  (\<G>, \<V>) \<Turnstile>\<^sub>\<E> \<E> \<Longrightarrow>
+  \<E> \<pi>\<^sub>r = Some (\<langle>LET x\<^sub>r = SYNC x\<^sub>r\<^sub>e in e\<^sub>r; \<rho>\<^sub>r; \<kappa>\<^sub>r\<rangle>) \<Longrightarrow>
+  (\<G>, \<V>) \<Turnstile>\<^sub>\<kappa>  \<V> (\<lfloor>e\<^sub>r\<rfloor>) \<Rrightarrow> \<kappa>\<^sub>r
+"
+ apply (erule accept_state_pool.cases, auto)
+ apply (drule spec[of _ \<pi>\<^sub>r])
+ apply (drule spec[of _ "\<langle>LET x\<^sub>r = SYNC x\<^sub>r\<^sub>e in e\<^sub>r; \<rho>\<^sub>r; \<kappa>\<^sub>r\<rangle>"], auto)
+ apply (erule accept_state.cases, auto) 
+done
+
+lemma flow_let_sync_preservation: "
+  (\<G>, \<V>) \<Turnstile>\<^sub>\<E> \<E> \<Longrightarrow>
+  \<E>' = \<E>(\<pi>\<^sub>s ;; x\<^sub>s \<mapsto> \<langle>e\<^sub>s; \<rho>\<^sub>s(x\<^sub>s \<mapsto> \<lbrace>\<rbrace>); \<kappa>\<^sub>s\<rangle>, \<pi>\<^sub>r ;; x\<^sub>r \<mapsto> \<langle>e\<^sub>r; \<rho>\<^sub>r(x\<^sub>r \<mapsto> \<omega>\<^sub>m); \<kappa>\<^sub>r\<rangle>) \<Longrightarrow>
+  leaf \<E> \<pi>\<^sub>s \<Longrightarrow>
+  \<E> \<pi>\<^sub>s = Some (\<langle>LET x\<^sub>s = SYNC x\<^sub>s\<^sub>e in e\<^sub>s; \<rho>\<^sub>s; \<kappa>\<^sub>s\<rangle>) \<Longrightarrow>
+  \<rho>\<^sub>s x\<^sub>s\<^sub>e = Some \<lbrace>Send_Evt x\<^sub>s\<^sub>c x\<^sub>m, \<rho>\<^sub>s\<^sub>e\<rbrace> \<Longrightarrow>
+  \<rho>\<^sub>s\<^sub>e x\<^sub>s\<^sub>c = Some \<lbrace>c\<rbrace> \<Longrightarrow>
+  \<rho>\<^sub>s\<^sub>e x\<^sub>m = Some \<omega>\<^sub>m \<Longrightarrow>
+  leaf \<E> \<pi>\<^sub>r \<Longrightarrow>
+  \<E> \<pi>\<^sub>r = Some (\<langle>LET x\<^sub>r = SYNC x\<^sub>r\<^sub>e in e\<^sub>r; \<rho>\<^sub>r; \<kappa>\<^sub>r\<rangle>) \<Longrightarrow>
+  \<rho>\<^sub>r x\<^sub>r\<^sub>e = Some \<lbrace>Recv_Evt x\<^sub>r\<^sub>c, \<rho>\<^sub>r\<^sub>e\<rbrace> \<Longrightarrow>
+  \<rho>\<^sub>r\<^sub>e x\<^sub>r\<^sub>c = Some \<lbrace>c\<rbrace> \<Longrightarrow> (\<G>, \<V>) \<Turnstile>\<^sub>\<E> \<E>(\<pi>\<^sub>s ;; x\<^sub>s \<mapsto> \<langle>e\<^sub>s; \<rho>\<^sub>s(x\<^sub>s \<mapsto> \<lbrace>\<rbrace>); \<kappa>\<^sub>s\<rangle>, \<pi>\<^sub>r ;; x\<^sub>r \<mapsto> \<langle>e\<^sub>r; \<rho>\<^sub>r(x\<^sub>r \<mapsto> \<omega>\<^sub>m); \<kappa>\<^sub>r\<rangle>)
+"
+ apply (rule accept_state_pool.Any, auto)
+     apply (rule accept_state.Any)
+      apply (erule flow_over_pool_to_exp_1, auto)
+     apply (erule flow_over_pool_to_env_1; (erule Pure.asm_rl)+)
+    apply (erule flow_over_pool_to_stack_1, auto)
+   apply (rule accept_state.Any)
+     apply (erule flow_over_pool_to_exp_1, auto)
+    apply ((erule flow_over_pool_to_env_1); (erule Pure.asm_rl)+)
+   apply (erule flow_over_pool_to_stack_1, auto)
+   apply (unfold not_def, erule impE, auto)
+   apply (rule accept_state.Any)
+   apply (erule flow_over_pool_to_exp_2, auto)
+     apply (erule flow_over_pool_to_env_2; (erule Pure.asm_rl)+)
+    apply (erule flow_over_pool_to_stack_2, auto)
+    apply (unfold not_def, erule impE, auto)
+    apply (rule accept_state.Any)
+     apply (erule flow_over_pool_to_exp_2, auto)
+    apply ((erule flow_over_pool_to_env_2); (erule Pure.asm_rl)+)
+   apply (erule flow_over_pool_to_stack_2; auto)
+  apply (erule accept_state_pool.cases; auto)
+done
+
+lemma flow_over_pool_to_exp_3: "
+  (\<G>, \<V>) \<Turnstile>\<^sub>\<E> \<E> \<Longrightarrow> \<E>' = \<E>(\<pi> ;; x \<mapsto> \<langle>e; \<rho>(x \<mapsto> \<lbrace>Ch \<pi> x\<rbrace>); \<kappa>\<rangle>) \<Longrightarrow> 
+  leaf \<E> \<pi> \<Longrightarrow> \<E> \<pi> = Some (\<langle>LET x = CHAN \<lparr>\<rparr> in e; \<rho>; \<kappa>\<rangle>) \<Longrightarrow> 
+  (\<G>, \<V>) \<Turnstile>\<^sub>e  e
+"
+ apply (erule accept_state_pool.cases, auto)
+ apply (drule spec[of _ \<pi>])
+ apply (drule spec[of _ "\<langle>LET x = CHAN \<lparr>\<rparr> in e; \<rho>; \<kappa>\<rangle>"], auto)
+ apply (erule accept_state.cases, auto)
+ apply (erule accept_exp.cases, auto)
+done
+
+lemma flow_over_pool_to_env_3: "
+  (\<G>, \<V>) \<Turnstile>\<^sub>\<E> \<E> \<Longrightarrow> \<E>' = \<E>(\<pi> ;; x \<mapsto> \<langle>e; \<rho>(x \<mapsto> \<lbrace>Ch \<pi> x\<rbrace>); \<kappa>\<rangle>) \<Longrightarrow> 
+  leaf \<E> \<pi> \<Longrightarrow> \<E> \<pi> = Some (\<langle>LET x = CHAN \<lparr>\<rparr> in e; \<rho>; \<kappa>\<rangle>) \<Longrightarrow> 
+  (\<G>, \<V>) \<Turnstile>\<^sub>\<rho> \<rho>(x \<mapsto> \<lbrace>Ch \<pi> x\<rbrace>)
+"
+ apply (rule accept_value_accept_val_env.Any, auto)
+      apply (erule accept_state_pool.cases, auto)
+      apply (drule spec[of _ \<pi>])
+      apply (drule spec[of _ "\<langle>LET x = CHAN \<lparr>\<rparr> in e; \<rho>; \<kappa>\<rangle>"], auto)
+      apply (erule accept_state.cases, auto)
+      apply (erule accept_exp.cases, auto)
+     apply (rule accept_value_accept_val_env.Chan)
+    apply (rename_tac x' \<omega>)
+    apply (erule accept_state_pool.cases, auto)
+    apply (drule spec[of _ \<pi>])
+    apply (drule spec[of _ "\<langle>LET x = CHAN \<lparr>\<rparr> in e; \<rho>; \<kappa>\<rangle>"], auto)
+    apply (erule accept_state.cases, auto)
+    apply (erule accept_exp.cases, auto)
+    apply (erule accept_val_env.cases, auto)
+   apply (rename_tac x' \<omega>)
+   apply (erule accept_state_pool.cases, auto)
+   apply (drule spec[of _ \<pi>])
+   apply (drule spec[of _ "\<langle>LET x = CHAN \<lparr>\<rparr> in e; \<rho>; \<kappa>\<rangle>"], auto)
+   apply (erule accept_state.cases, auto)
+   apply (erule accept_exp.cases, auto)
+   apply (erule accept_val_env.cases, auto)
+done
+
+lemma flow_over_pool_to_stack_3: "
+  (\<G>, \<V>) \<Turnstile>\<^sub>\<E> \<E> \<Longrightarrow> \<E>' = \<E>(\<pi> ;; x \<mapsto> \<langle>e; \<rho>(x \<mapsto> \<lbrace>Ch \<pi> x\<rbrace>); \<kappa>\<rangle>) \<Longrightarrow> leaf \<E> \<pi> \<Longrightarrow> \<E> \<pi> = Some (\<langle>LET x = CHAN \<lparr>\<rparr> in e; \<rho>; \<kappa>\<rangle>) \<Longrightarrow> (\<G>, \<V>) \<Turnstile>\<^sub>\<kappa>  \<V> (\<lfloor>e\<rfloor>) \<Rrightarrow> \<kappa>
+"
+ apply (erule accept_state_pool.cases, auto)
+ apply (drule spec[of _ \<pi>])
+ apply (drule spec[of _ "\<langle>LET x = CHAN \<lparr>\<rparr> in e; \<rho>; \<kappa>\<rangle>"], auto)
+ apply (erule accept_state.cases, auto)
+done
+
+lemma flow_over_pool_to_exp_4: "
+  (\<G>, \<V>) \<Turnstile>\<^sub>\<E> \<E> \<Longrightarrow> \<E>' = \<E>(\<pi> ;; x \<mapsto> \<langle>e; \<rho>(x \<mapsto> \<lbrace>Ch \<pi> x\<rbrace>); \<kappa>\<rangle>) \<Longrightarrow>
+  leaf \<E> \<pi> \<Longrightarrow> \<E> \<pi> = Some (\<langle>LET x = CHAN \<lparr>\<rparr> in e; \<rho>; \<kappa>\<rangle>) \<Longrightarrow> \<pi>' \<noteq> \<pi> ;; x \<Longrightarrow> \<E> \<pi>' = Some (\<langle>e'; \<rho>'; \<kappa>'\<rangle>) \<Longrightarrow> 
+  (\<G>, \<V>) \<Turnstile>\<^sub>e  e'
+"
+ apply (erule accept_state_pool.cases, auto)
+ apply (drule spec[of _ \<pi>'])
+ apply (drule spec[of _ "\<langle>e'; \<rho>'; \<kappa>'\<rangle>"], auto)
+ apply (erule accept_state.cases, auto)
+done
+
+lemma flow_over_pool_to_env_4: "
+  (\<G>, \<V>) \<Turnstile>\<^sub>\<E> \<E> \<Longrightarrow> \<E>' = \<E>(\<pi> ;; x \<mapsto> \<langle>e; \<rho>(x \<mapsto> \<lbrace>Ch \<pi> x\<rbrace>); \<kappa>\<rangle>) \<Longrightarrow>
+  leaf \<E> \<pi> \<Longrightarrow> \<E> \<pi> = Some (\<langle>LET x = CHAN \<lparr>\<rparr> in e; \<rho>; \<kappa>\<rangle>) \<Longrightarrow> \<pi>' \<noteq> \<pi> ;; x \<Longrightarrow> \<E> \<pi>' = Some (\<langle>e'; \<rho>'; \<kappa>'\<rangle>) \<Longrightarrow> 
+  (\<G>, \<V>) \<Turnstile>\<^sub>\<rho> \<rho>'
+"
+ apply (rule accept_value_accept_val_env.Any, auto)
+    apply (erule accept_state_pool.cases, auto)
+    apply (drule spec[of _ \<pi>'])
+    apply (drule spec[of _ "\<langle>e'; \<rho>'; \<kappa>'\<rangle>"], auto)
+    apply (erule accept_state.cases, auto)
+    apply (erule accept_val_env.cases, auto)
+   apply (erule accept_state_pool.cases, auto)
+   apply (drule spec[of _ \<pi>'])
+   apply (drule spec[of _ "\<langle>e'; \<rho>'; \<kappa>'\<rangle>"], auto)
+   apply (erule accept_state.cases, auto)
+   apply (erule accept_val_env.cases, auto)
+done
+
+lemma flow_over_pool_to_stack_4: "
+  (\<G>, \<V>) \<Turnstile>\<^sub>\<E> \<E> \<Longrightarrow> \<E>' = \<E>(\<pi> ;; x \<mapsto> \<langle>e; \<rho>(x \<mapsto> \<lbrace>Ch \<pi> x\<rbrace>); \<kappa>\<rangle>) \<Longrightarrow>
+  leaf \<E> \<pi> \<Longrightarrow> \<E> \<pi> = Some (\<langle>LET x = CHAN \<lparr>\<rparr> in e; \<rho>; \<kappa>\<rangle>) \<Longrightarrow> \<pi>' \<noteq> \<pi> ;; x \<Longrightarrow> \<E> \<pi>' = Some (\<langle>e'; \<rho>'; \<kappa>'\<rangle>) \<Longrightarrow> 
+  (\<G>, \<V>) \<Turnstile>\<^sub>\<kappa>  \<V> (\<lfloor>e'\<rfloor>) \<Rrightarrow> \<kappa>'
+"
+ apply (erule accept_state_pool.cases, auto)
+ apply (drule spec[of _ \<pi>'])
+ apply (drule spec[of _ "\<langle>e'; \<rho>'; \<kappa>'\<rangle>"], auto)
+ apply (erule accept_state.cases, auto)
+done
+
+lemma flow_let_chan_preservation: "
+  (\<G>, \<V>) \<Turnstile>\<^sub>\<E> \<E> \<Longrightarrow> \<E>' = \<E>(\<pi> ;; x \<mapsto> \<langle>e; \<rho>(x \<mapsto> \<lbrace>Ch \<pi> x\<rbrace>); \<kappa>\<rangle>) \<Longrightarrow> 
+  leaf \<E> \<pi> \<Longrightarrow> \<E> \<pi> = Some (\<langle>LET x = CHAN \<lparr>\<rparr> in e; \<rho>; \<kappa>\<rangle>) \<Longrightarrow> 
+  (\<G>, \<V>) \<Turnstile>\<^sub>\<E> \<E>(\<pi> ;; x \<mapsto> \<langle>e; \<rho>(x \<mapsto> \<lbrace>Ch \<pi> x\<rbrace>); \<kappa>\<rangle>)
+"
+ apply (rule accept_state_pool.Any, auto)
+  apply (rule accept_state.Any)
+    apply (erule flow_over_pool_to_exp_3, auto)
+   apply (erule flow_over_pool_to_env_3, auto)
+  apply (erule flow_over_pool_to_stack_3, auto)
+ apply (case_tac "\<sigma>", rename_tac e' \<rho>' \<kappa>', auto)
+ apply (rule accept_state.Any)
+   apply (erule flow_over_pool_to_exp_4, auto)
+   apply (erule flow_over_pool_to_env_4, auto)
+  apply (erule flow_over_pool_to_stack_4, auto)
+done
+
+
+lemma flow_over_pool_to_exp_5: "
+  (\<G>, \<V>) \<Turnstile>\<^sub>\<E> \<E> \<Longrightarrow> \<E>' = \<E>(\<pi> ;; x \<mapsto> \<langle>e; \<rho>(x \<mapsto> \<lbrace>\<rbrace>); \<kappa>\<rangle>, \<pi>;;.x \<mapsto> \<langle>e\<^sub>c; \<rho>; []\<rangle>) \<Longrightarrow> 
+  leaf \<E> \<pi> \<Longrightarrow> \<E> \<pi> = Some (\<langle>LET x = SPAWN e\<^sub>c in e; \<rho>; \<kappa>\<rangle>) \<Longrightarrow> 
+  (\<G>, \<V>) \<Turnstile>\<^sub>e  e
+"
+ apply (erule accept_state_pool.cases, auto)
+ apply (drule spec[of _ \<pi>])
+ apply (drule spec[of _ "\<langle>LET x = SPAWN e\<^sub>c in e; \<rho>; \<kappa>\<rangle>"], auto)
+ apply (erule accept_state.cases, auto)
+ apply (erule accept_exp.cases, auto)
+done
+
+lemma flow_over_pool_to_env_5: "
+  (\<G>, \<V>) \<Turnstile>\<^sub>\<E> \<E> \<Longrightarrow> \<E>' = \<E>(\<pi> ;; x \<mapsto> \<langle>e; \<rho>(x \<mapsto> \<lbrace>\<rbrace>); \<kappa>\<rangle>, \<pi>;;.x \<mapsto> \<langle>e\<^sub>c; \<rho>; []\<rangle>) \<Longrightarrow> 
+  leaf \<E> \<pi> \<Longrightarrow> \<E> \<pi> = Some (\<langle>LET x = SPAWN e\<^sub>c in e; \<rho>; \<kappa>\<rangle>) \<Longrightarrow> 
+  (\<G>, \<V>) \<Turnstile>\<^sub>\<rho> \<rho>(x \<mapsto> \<lbrace>\<rbrace>)"
+ apply (rule accept_value_accept_val_env.Any, auto)
+      apply (erule accept_state_pool.cases, auto)
+      apply (drule spec[of _ \<pi>])
+      apply (drule spec[of _ "\<langle>LET x = SPAWN e\<^sub>c in e; \<rho>; \<kappa>\<rangle>"], auto)
+      apply (erule accept_state.cases, auto)
+      apply (erule accept_exp.cases, auto)
+     apply (rule accept_value_accept_val_env.Unit)
+    apply (rename_tac x' \<omega>)
+    apply (erule accept_state_pool.cases, auto)
+    apply (drule spec[of _ \<pi>])
+    apply (drule spec[of _ "\<langle>LET x = SPAWN e\<^sub>c in e; \<rho>; \<kappa>\<rangle>"], auto)
+    apply (erule accept_state.cases, auto)
+    apply (erule accept_exp.cases, auto)
+    apply (erule accept_val_env.cases, auto)
+   apply (rename_tac x' \<omega>)
+   apply (erule accept_state_pool.cases, auto)
+   apply (drule spec[of _ \<pi>])
+   apply (drule spec[of _ "\<langle>LET x = SPAWN e\<^sub>c in e; \<rho>; \<kappa>\<rangle>"], auto)
+   apply (erule accept_state.cases, auto)
+   apply (erule accept_exp.cases, auto)
+   apply (erule accept_val_env.cases, auto)
+done
+
+lemma flow_over_pool_to_stack_5: "
+  (\<G>, \<V>) \<Turnstile>\<^sub>\<E> \<E> \<Longrightarrow> \<E>' = \<E>(\<pi> ;; x \<mapsto> \<langle>e; \<rho>(x \<mapsto> \<lbrace>\<rbrace>); \<kappa>\<rangle>, \<pi>;;.x \<mapsto> \<langle>e\<^sub>c; \<rho>; []\<rangle>) \<Longrightarrow> 
+  leaf \<E> \<pi> \<Longrightarrow> \<E> \<pi> = Some (\<langle>LET x = SPAWN e\<^sub>c in e; \<rho>; \<kappa>\<rangle>) \<Longrightarrow> 
+  (\<G>, \<V>) \<Turnstile>\<^sub>\<kappa>  \<V> (\<lfloor>e\<rfloor>) \<Rrightarrow> \<kappa>
+"
+ apply (erule accept_state_pool.cases, auto)
+ apply (drule spec[of _ \<pi>])
+ apply (drule spec[of _ "\<langle>LET x = SPAWN e\<^sub>c in e; \<rho>; \<kappa>\<rangle>"], auto)
+ apply (erule accept_state.cases, auto)
+done
+
+lemma flow_over_pool_to_exp_6: "
+  (\<G>, \<V>) \<Turnstile>\<^sub>\<E> \<E> \<Longrightarrow> \<E>' = \<E>(\<pi> ;; x \<mapsto> \<langle>e; \<rho>(x \<mapsto> \<lbrace>\<rbrace>); \<kappa>\<rangle>, \<pi>;;.x \<mapsto> \<langle>e\<^sub>c; \<rho>; []\<rangle>) \<Longrightarrow> 
+  leaf \<E> \<pi> \<Longrightarrow> \<E> \<pi> = Some (\<langle>LET x = SPAWN e\<^sub>c in e; \<rho>; \<kappa>\<rangle>) \<Longrightarrow> 
+  (\<G>, \<V>) \<Turnstile>\<^sub>e  e\<^sub>c
+"   
+ apply (erule accept_state_pool.cases, auto)
+ apply (drule spec[of _ \<pi>])
+ apply (drule spec[of _ "\<langle>LET x = SPAWN e\<^sub>c in e; \<rho>; \<kappa>\<rangle>"], auto)
+ apply (erule accept_state.cases, auto)
+ apply (erule accept_exp.cases, auto)
+done
+
+lemma flow_over_pool_to_env_6: "
+  (\<G>, \<V>) \<Turnstile>\<^sub>\<E> \<E> \<Longrightarrow> \<E>' = \<E>(\<pi> ;; x \<mapsto> \<langle>e; \<rho>(x \<mapsto> \<lbrace>\<rbrace>); \<kappa>\<rangle>, \<pi>;;.x \<mapsto> \<langle>e\<^sub>c; \<rho>; []\<rangle>) \<Longrightarrow> 
+  leaf \<E> \<pi> \<Longrightarrow> \<E> \<pi> = Some (\<langle>LET x = SPAWN e\<^sub>c in e; \<rho>; \<kappa>\<rangle>) \<Longrightarrow> 
+  (\<G>, \<V>) \<Turnstile>\<^sub>\<rho> \<rho>
+"   
+ apply (erule accept_state_pool.cases, auto)
+ apply (drule spec[of _ \<pi>])
+ apply (drule spec[of _ "\<langle>LET x = SPAWN e\<^sub>c in e; \<rho>; \<kappa>\<rangle>"], auto)
+ apply (erule accept_state.cases, auto)
+done
+
+lemma flow_over_pool_to_stack_6: "
+  (\<G>, \<V>) \<Turnstile>\<^sub>\<E> \<E> \<Longrightarrow> \<E>' = \<E>(\<pi> ;; x \<mapsto> \<langle>e; \<rho>(x \<mapsto> \<lbrace>\<rbrace>); \<kappa>\<rangle>, \<pi>;;.x \<mapsto> \<langle>e\<^sub>c; \<rho>; []\<rangle>) \<Longrightarrow> 
+  leaf \<E> \<pi> \<Longrightarrow> \<E> \<pi> = Some (\<langle>LET x = SPAWN e\<^sub>c in e; \<rho>; \<kappa>\<rangle>) \<Longrightarrow> 
+  (\<G>, \<V>) \<Turnstile>\<^sub>\<kappa>  \<V> (\<lfloor>e\<^sub>c\<rfloor>) \<Rrightarrow> []
+"   
+ apply (rule accept_stack.Empty)
+done
+
+
+lemma flow_let_spawn_preservation: "
+  (\<G>, \<V>) \<Turnstile>\<^sub>\<E> \<E> \<Longrightarrow> \<E>' = \<E>(\<pi> ;; x \<mapsto> \<langle>e; \<rho>(x \<mapsto> \<lbrace>\<rbrace>); \<kappa>\<rangle>, \<pi>;;.x \<mapsto> \<langle>e\<^sub>c; \<rho>; []\<rangle>) \<Longrightarrow>
+  leaf \<E> \<pi> \<Longrightarrow> \<E> \<pi> = Some (\<langle>LET x = SPAWN e\<^sub>c in e; \<rho>; \<kappa>\<rangle>) \<Longrightarrow> 
+  (\<G>, \<V>) \<Turnstile>\<^sub>\<E> \<E>(\<pi> ;; x \<mapsto> \<langle>e; \<rho>(x \<mapsto> \<lbrace>\<rbrace>); \<kappa>\<rangle>, \<pi>;;.x \<mapsto> \<langle>e\<^sub>c; \<rho>; []\<rangle>)
+"
+  apply (rule accept_state_pool.Any, auto)
+    apply (rule accept_state.Any)
+     apply (erule flow_over_pool_to_exp_5, auto)
+    apply (erule flow_over_pool_to_env_5, auto)
+   apply (erule flow_over_pool_to_stack_5, auto)
+   apply (unfold not_def, erule impE, auto)
+   apply (rule accept_state.Any)
+     apply (erule flow_over_pool_to_exp_6, auto)
+    apply (erule flow_over_pool_to_env_6, auto)
+   apply (erule flow_over_pool_to_stack_6, auto)
+  apply (erule accept_state_pool.cases, auto)
+done
+
+
+*)
+(*******)
+theorem flow_preservation : "
+  \<lbrakk>
+    (\<G>, \<V>) \<Turnstile>\<^sub>\<E> \<E>; 
+    \<E> \<rightarrow> \<E>'
+  \<rbrakk> \<Longrightarrow>
+  (\<G>, \<V>) \<Turnstile>\<^sub>\<E> \<E>'
+"
+ apply (erule concur_step.cases, auto)
+    apply (erule flow_seq_step_preservation, auto)
+   apply ((erule flow_let_sync_preservation; blast?), auto)
+  apply (erule flow_let_chan_preservation, auto)
+ apply (erule flow_let_spawn_preservation, auto)
+sorry
+
+
+theorem flow_preservation_star' : "
+  \<E> \<rightarrow>* \<E>' \<Longrightarrow>
+  ((\<G>, \<V>) \<Turnstile>\<^sub>\<E> \<E> \<longrightarrow> (\<G>, \<V>) \<Turnstile>\<^sub>\<E> \<E>')
+"
+ apply (erule star.induct[of concur_step], auto)
+ apply (rename_tac \<E> \<E>' \<E>'')
+ apply (erule notE)
+ apply (erule flow_preservation, auto)
+done
+ 
+
+theorem flow_preservation_star : "
+  \<lbrakk>
+    (\<G>, \<V>) \<Turnstile>\<^sub>\<E> \<E>;  
+    \<E> \<rightarrow>* \<E>'
+  \<rbrakk> \<Longrightarrow>
+  (\<G>, \<V>) \<Turnstile>\<^sub>\<E> \<E>'
+"
+by (drule flow_preservation_star', auto)
+
+theorem flow_over_env_precision : "
+  (\<G>, \<V>) \<Turnstile>\<^sub>\<rho> \<rho>
+  \<Longrightarrow>
+  \<parallel>\<rho>\<parallel> \<sqsubseteq> \<V>
+"
+ apply (unfold abstract_value_env_precision_def, unfold env_to_abstract_value_env_def)
+ apply (rule allI, rename_tac x)
+ apply (case_tac "\<rho> x = None", auto, rename_tac \<omega>)
+ apply (erule accept_val_env.cases, auto)
+done
+
+theorem flow_over_state_precision : "
+  (\<G>, \<V>) \<Turnstile>\<^sub>\<sigma> \<langle>e; \<rho>; \<kappa>\<rangle>
+  \<Longrightarrow>
+  \<parallel>\<rho>\<parallel> \<sqsubseteq> \<V>
+"
+ apply (erule accept_state.cases, auto)
+ apply (erule flow_over_env_precision)
+done
+
+lemma flow_over_pool_to_state: "
+  \<lbrakk>
+    (\<G>, \<V>) \<Turnstile>\<^sub>\<E> \<E>; 
+    \<E> \<pi> = Some \<sigma> 
+  \<rbrakk>
+  \<Longrightarrow>
+  (\<G>, \<V>) \<Turnstile>\<^sub>\<sigma>  \<sigma>
+"
+ apply (erule accept_state_pool.cases)
+ apply (drule spec[of _ \<pi>])
+ apply (drule spec[of _ \<sigma>])
+ apply (erule impE, auto)
+done
+
+  
+theorem flow_over_pool_precision : "
+  \<lbrakk>
+    (\<G>, \<V>) \<Turnstile>\<^sub>\<E> \<E>;
+    \<E> \<pi> = Some (\<langle>e; \<rho>; \<kappa>\<rangle>)
+  \<rbrakk>
+  \<Longrightarrow>
+  \<parallel>\<rho>\<parallel> \<sqsubseteq> \<V>
+"
+ apply (drule flow_over_pool_to_state, simp)
+ apply (erule flow_over_state_precision)
+done
+
+theorem lift_flow_exp_to_state: "(\<G>, \<V>) \<Turnstile>\<^sub>e e \<Longrightarrow> (\<G>, \<V>) \<Turnstile>\<^sub>\<sigma>  \<langle>e; empty; []\<rangle>"
+ apply (rule accept_state.Any, auto)
+ apply (rule+, auto, rule)
+done
+
+theorem  lift_flow_state_to_pool: "(\<G>, \<V>) \<Turnstile>\<^sub>\<sigma>  \<sigma> \<Longrightarrow> (\<G>, \<V>) \<Turnstile>\<^sub>\<E> [[] \<mapsto> \<sigma>]"
+  apply (rule accept_state_pool.Any)
+  apply (case_tac "\<pi> = []", auto)
+done
+
+theorem lift_flow_exp_to_pool: "(\<G>, \<V>) \<Turnstile>\<^sub>e  e \<Longrightarrow> (\<G>, \<V>) \<Turnstile>\<^sub>\<E> [[] \<mapsto> \<langle>e; empty; []\<rangle>]"
+  apply (drule lift_flow_exp_to_state)
+  apply (erule lift_flow_state_to_pool)
+done
+
+theorem flow_over_pool_sound : "
+  \<lbrakk>
+    (\<G>, \<V>) \<Turnstile>\<^sub>\<E> \<E>; 
+    \<E> \<rightarrow>* \<E>';
+    \<E>' \<pi> = Some (\<langle>e'; \<rho>'; \<kappa>'\<rangle>)
+  \<rbrakk> \<Longrightarrow>
+  \<parallel>\<rho>'\<parallel> \<sqsubseteq> \<V>
+"
+ apply (drule flow_preservation_star[of \<G> \<V> _ \<E>'], auto)
+ apply (erule flow_over_pool_precision[of \<G> \<V> \<E>' \<pi> e' \<rho>' \<kappa>'], auto)
+done
+
+theorem flow_sound : "
+  \<lbrakk>
+    (\<G>, \<V>) \<Turnstile>\<^sub>e e; 
+    [[] \<mapsto> \<langle>e; empty; []\<rangle>] \<rightarrow>* \<E>';
+    \<E>' \<pi> = Some (\<langle>e'; \<rho>'; \<kappa>'\<rangle>)
+  \<rbrakk> \<Longrightarrow>
+  \<parallel>\<rho>'\<parallel> \<sqsubseteq> \<V>
+"
+ apply (drule lift_flow_exp_to_pool)
+ apply (erule flow_over_pool_sound [of \<G> \<V> _ \<E>' \<pi> e' \<rho>' \<kappa>'], auto)
+done
+
+corollary flow_sound_coro: "
+  \<lbrakk>
+    (\<G>, \<V>) \<Turnstile>\<^sub>e e ;
+    [[] \<mapsto> \<langle>e;Map.empty;[]\<rangle>] \<rightarrow>* \<E>';
+    \<E>' \<pi> = Some (\<langle>e';\<rho>';\<kappa>'\<rangle>);
+    \<rho>' x = Some \<omega>
+  \<rbrakk> \<Longrightarrow>
+  {|\<omega>|} \<subseteq> \<V> x
+"
+  apply (drule flow_sound; assumption?)
+  apply (unfold abstract_value_env_precision_def)
+  apply (unfold env_to_abstract_value_env_def)
+  apply (drule spec[of _ x]; auto)
+done
+
+
+
+
+
+
+end
+
+
+
+(*****)
+
 inductive accept_exp :: "abstract_value_env \<times> abstract_value_env \<times> bind_env \<Rightarrow> exp \<Rightarrow> bool" (infix "\<Turnstile>\<^sub>e" 55) where
   Result: "
     (\<V>, \<C>, \<X>) \<Turnstile>\<^sub>e (RESULT x)
